@prefix amsl: <http://vocab.ub.uni-leipzig.de/amsl/> .

@prefix aiiso: <http://purl.org/vocab/aiiso/schema#> .
@prefix bibo: <http://purl.org/ontology/bibo/> .
@prefix cc: <http://creativecommons.org/ns#> .
@prefix count: <http://vocab.ub.uni-leipzig.de/counter/> .
@prefix dc: <http://purl.org/dc/elements/1.1/> .
@prefix dct:  <http://purl.org/dc/terms/> .
@prefix doap: <http://usefulinc.com/ns/doap#> .
@prefix foaf: <http://xmlns.com/foaf/0.1/> .
@prefix gr: <http://purl.org/goodrelations/v1#> .
@prefix lobid: <http://purl.org/lobid/lv#> .
@prefix owl: <http://www.w3.org/2002/07/owl#> .
@prefix rdf: <http://www.w3.org/1999/02/22-rdf-syntax-ns#> .
@prefix rdfs: <http://www.w3.org/2000/01/rdf-schema#> .
@prefix rdvocab: <http://rdaregistry.info/> .
@prefix sioc: <http://rdfs.org/sioc/ns#> .
@prefix skos: <http://www.w3.org/2004/02/skos/core#> .
@prefix sushi: <http://vocab.ub.uni-leipzig.de/sushi/> .
@prefix sysont: <http://ns.ontowiki.net/SysOnt/> .
@prefix terms: <http://vocab.ub.uni-leipzig.de/terms/> .
@prefix vann: <http://purl.org/vocab/vann/> .
@prefix vcard: <http://www.w3.org/2006/vcard/ns#> .
@prefix xml: <http://www.w3.org/XML/1998/namespace> .
@prefix xsd: <http://www.w3.org/2001/XMLSchema#> .

amsl: a owl:Ontology ;
    rdfs:label "amsl Vocabulary for Library Electronic Resource Management"@en , "amsl-Vokabular für Electronic Resource Management in Bibliotheken"@de ;
    cc:attributionName "AKSW & Universitätsbibliothek Leipzig" ;
    vann:changes <https://github.com/amsl-project/amsl.vocab/commits/master> ;
    vann:preferredNamespacePrefix "amsl" ;
    vann:preferredNamespaceUri "http://vocab.ub.uni-leipzig.de/amsl/" ;
    doap:homepage <http://amsl.technology> ;
    doap:maintainer <http://aksw.org/Partner/AnnikaDomin> ;
    foaf:maker 
        <http://aksw.org/NatanaelArndt>,
        <http://aksw.org/Partner/AnnikaDomin>,
        <http://aksw.org/Partner/BjoernMuschall>,
        <http://aksw.org/AndreasNareike> ,
        <http://aksw.org/SebastianNuck> ,
        <http://aksw.org/NormanRadtke>,
        <http://aksw.org/ThomasRiechert> ,
        <http://aksw.org/Partner/LydiaUnterdoerfel> .


######################## Classes #####################################

amsl:AnnualBudget a owl:Class ;
    rdfs:label "Jahresbudget"@de ,
        "Annual Budget"@en ;
    rdfs:subClassOf 
        [   a owl:restriction ;
            owl:onProperty amsl:budget ;
            owl:cardinality "1"^^xsd:nonNegativeInteger ] ,
        [   a owl:restriction ;
            owl:onProperty amsl:fiscalYear ;
            owl:cardinality "1"^^xsd:nonNegativeInteger ] ,
        [   a owl:restriction ;
            owl:onProperty rdfs:label ;
            owl:cardinality "1"^^xsd:nonNegativeInteger ] ;
    rdfs:comment "Ein auf bestimmtes Haushaltsjahr bezogenes Budget."@de ,
        "A budget for a certain fiscal year."@en .

amsl:AnnualContractData a owl:Class ;
    rdfs:label "Vertragsjahresdaten"@de ,
        "Annual Contract Data"@en ;
    rdfs:subClassOf 
        amsl:ContractData ,
        [   a owl:restriction ;
            owl:onProperty amsl:annualBudget ;
            owl:minCardinality "1"^^xsd:nonNegativeInteger ] ,
        [   a owl:restriction ;
            owl:onProperty amsl:annualPrice ;
            owl:maxCardinality "1"^^xsd:nonNegativeInteger  ] ,
        [   a owl:restriction ;
            owl:onProperty amsl:balanceFile ;
            owl:minCardinality "0"^^xsd:nonNegativeInteger ] ,
        [   a owl:restriction ;
            owl:onProperty amsl:basicContractData ;
            owl:cardinality "1"^^xsd:nonNegativeInteger  ] ,
        # amsl:budget nicht mit aufgenommen, da durch annual budget zu ersetzen.
        [   a owl:restriction ;
            owl:onProperty amsl:contractFile ;
            owl:minCardinality "0"^^xsd:nonNegativeInteger ] ,
        [   a owl:restriction ;
            owl:onProperty amsl:expectedInvoiceDate  ;
            owl:maxCardinality "1"^^xsd:nonNegativeInteger  ] ,
        [   a owl:restriction ;
            owl:onProperty amsl:expectedPrice  ;
            owl:maxCardinality "1"^^xsd:nonNegativeInteger  ] ,
        [   a owl:restriction ;
            owl:onProperty amsl:expectedPriceSubtotal ;
            owl:minCardinality "0"^^xsd:nonNegativeInteger  ] ,
        [   a owl:restriction ;
            owl:onProperty amsl:externalContact ;
            owl:minCardinality "0"^^xsd:nonNegativeInteger  ] ,
        [   a owl:restriction ;
            owl:onProperty amsl:facultyShare ;
            owl:minCardinality "0"^^xsd:nonNegativeInteger  ] ,
        [   a owl:restriction ;
            owl:onProperty amsl:feedbackDate  ;
            owl:maxCardinality "1"^^xsd:nonNegativeInteger  ] ,
        [   a owl:restriction ;
            owl:onProperty amsl:file ;
            owl:minCardinality "0"^^xsd:nonNegativeInteger  ] ,
        [   a owl:restriction ;
            owl:onProperty amsl:invoiceDate  ;
            owl:maxCardinality "1"^^xsd:nonNegativeInteger  ] ,
        [   a owl:restriction ;
            owl:onProperty amsl:invoiceFile ;
            owl:minCardinality "0"^^xsd:nonNegativeInteger  ] ,
        [   a owl:restriction ;
            owl:onProperty amsl:invoicePriceGrossEUR  ;
            owl:maxCardinality "1"^^xsd:nonNegativeInteger  ] ,
        [   a owl:restriction ;
            owl:onProperty amsl:invoicePriceGrossGBP  ;
            owl:maxCardinality "1"^^xsd:nonNegativeInteger  ] ,
        [   a owl:restriction ;
            owl:onProperty amsl:invoicePriceGrossUSD  ;
            owl:maxCardinality "1"^^xsd:nonNegativeInteger  ] ,
        [   a owl:restriction ;
            owl:onProperty amsl:invoicePriceNetEUR  ;
            owl:maxCardinality "1"^^xsd:nonNegativeInteger  ] ,
        [   a owl:restriction ;
            owl:onProperty amsl:invoicePriceNetGBP  ;
            owl:maxCardinality "1"^^xsd:nonNegativeInteger  ] ,
        [   a owl:restriction ;
            owl:onProperty amsl:invoicePriceNetUSD  ;
            owl:maxCardinality "1"^^xsd:nonNegativeInteger  ] ,
        [   a owl:restriction ;
            owl:onProperty amsl:invoicePriceSubtotal ;
            owl:minCardinality "0"^^xsd:nonNegativeInteger  ] ,
        [   a owl:restriction ;
            owl:onProperty amsl:invoiceProcessingDate  ;
            owl:maxCardinality "1"^^xsd:nonNegativeInteger  ] ,
        [   a owl:restriction ;
            owl:onProperty amsl:invoiceReceived  ;
            owl:cardinality "1"^^xsd:nonNegativeInteger  ] ,
        [   a owl:restriction ;
            owl:onProperty amsl:licenseEndDate  ;
            owl:maxCardinality "1"^^xsd:nonNegativeInteger  ] ,
        [   a owl:restriction ;
            owl:onProperty amsl:licenseStartDate ;
            owl:cardinality "1"^^xsd:nonNegativeInteger  ] ,
        [   a owl:restriction ;
            owl:onProperty amsl:licenseType  ;
            owl:cardinality "1"^^xsd:nonNegativeInteger  ] ,
        [   a owl:restriction ;
            owl:onProperty amsl:licensingAgent ;
            owl:maxCardinality "1"^^xsd:nonNegativeInteger  ] ,
        [   a owl:restriction ;
            owl:onProperty amsl:licensingNote ;
            owl:minCardinality "0"^^xsd:nonNegativeInteger  ] ,
        [   a owl:restriction ;
            owl:onProperty amsl:linkToBalance ;
            owl:minCardinality "0"^^xsd:nonNegativeInteger  ] ,
        [   a owl:restriction ;
            owl:onProperty amsl:linkToContract ;
            owl:minCardinality "0"^^xsd:nonNegativeInteger  ] ,
        [   a owl:restriction ;
            owl:onProperty amsl:linkToInvoice ;
            owl:minCardinality "0"^^xsd:nonNegativeInteger  ] ,
        [   a owl:restriction ;
            owl:onProperty amsl:localSystemNumber ;
            owl:minCardinality "0"^^xsd:nonNegativeInteger  ] ,
        [   a owl:restriction ;
            owl:onProperty amsl:mailFile ;
            owl:minCardinality "0"^^xsd:nonNegativeInteger  ] ,
        [   a owl:restriction ;
            owl:onProperty amsl:noticePeriod ;
            owl:maxCardinality "1"^^xsd:nonNegativeInteger  ] ,
        [   a owl:restriction ;
            owl:onProperty amsl:paymentPeriod ;
            owl:maxCardinality "1"^^xsd:nonNegativeInteger  ] ,
        [   a owl:restriction ;
            owl:onProperty amsl:terminationAlert ;
            owl:maxCardinality "1"^^xsd:nonNegativeInteger  ] ,
        [   a owl:restriction ;
            owl:onProperty amsl:usageStatsNote ;
            owl:minCardinality "0"^^xsd:nonNegativeInteger  ] ,
        [   a owl:restriction ;
            owl:onProperty amsl:workflowStatus ;
            owl:minCardinality "0"^^xsd:nonNegativeInteger ;
            owl:maxCardinality "1"^^xsd:nonNegativeInteger  ] ,
        [   a owl:restriction ;
            owl:onProperty rdfs:comment  ;
            owl:minCardinality "0"^^xsd:nonNegativeInteger  ] ,
        [   a owl:restriction ;
            owl:onProperty rdfs:label ;
            owl:minCardinality "1"^^xsd:nonNegativeInteger  ] ;
    rdfs:comment "Ein Geschäftsvertrag zwischen der Bibliothek und weiteren Perteien. Dieser Vertragsteil beinhaltet die sich jährlich ändernden Eigenschaften eines Vertrags."@de ,
        "A class modeling a business contract between the library and one or more parties. This part of the contract contains the annual (dynamic) properties of a contract."@en ;
    rdfs:seeAlso "ERMI terms: _Acquisition Entity_ (cf. https://old.diglib.org/pubs/dlf102/ERMFINAL.pdf, p. 141)" ;
    rdfs:seeAlso "ERMI terms: _License Entity_ (cf. https://old.diglib.org/pubs/dlf102/ERMFINAL.pdf, p. 144)" .

amsl:BasicContractData a owl:Class ;
    rdfs:label "Vertragsbasisdaten"@de ,
        "Basic Contract Data"@en ;
    rdfs:subClassOf 
        amsl:ContractData ,
        [   a owl:restriction ;
            owl:onProperty amsl:acqMethod ;
            owl:cardinality "1"^^xsd:nonNegativeInteger ] ,
        [   a owl:restriction ;
            owl:onProperty amsl:archivedAnnualContractDataLabel ;
            owl:minCardinality "0"^^xsd:nonNegativeInteger  ] ,
        [   a owl:restriction ;
            owl:onProperty amsl:archivingNote ;
            owl:minCardinality "0"^^xsd:nonNegativeInteger ] ,
        [   a owl:restriction ;
            owl:onProperty amsl:authMethod ;
            owl:cardinality "1"^^xsd:nonNegativeInteger ] ,
        [   a owl:restriction ;
            owl:onProperty amsl:authorizedUser ;
            owl:minCardinality "1"^^xsd:nonNegativeInteger ] ,
        [   a owl:restriction ;
            owl:onProperty amsl:concUser ;
            owl:maxCardinality "1"^^xsd:nonNegativeInteger ] ,
        [   a owl:restriction ;
            owl:onProperty amsl:consortium ;
            owl:maxCardinality "1"^^xsd:nonNegativeInteger ] ,
        [   a owl:restriction ;
            owl:onProperty amsl:consortiumLeader ;
            owl:maxCardinality "1"^^xsd:nonNegativeInteger ] ,
        [   a owl:restriction ;
            owl:onProperty amsl:contractFile ;
            owl:minCardinality "0"^^xsd:nonNegativeInteger ] ,
        [   a owl:restriction ;
            owl:onProperty amsl:coursePackE ;
            owl:maxCardinality "1"^^xsd:nonNegativeInteger ] ,
        [   a owl:restriction ;
            owl:onProperty amsl:coursePackP ;
            owl:maxCardinality "1"^^xsd:nonNegativeInteger ] ,
        [   a owl:restriction ;
            owl:onProperty amsl:courseReserveE ;
            owl:maxCardinality "1"^^xsd:nonNegativeInteger ] ,
        [   a owl:restriction ;
            owl:onProperty amsl:courseReserveP ;
            owl:maxCardinality "1"^^xsd:nonNegativeInteger ] ,
        [   a owl:restriction ;
            owl:onProperty amsl:dataAvailability ;
            owl:minCardinality "0"^^xsd:nonNegativeInteger ] ,
        [   a owl:restriction ;
            owl:onProperty amsl:dbType ;
            owl:minCardinality "0"^^xsd:nonNegativeInteger ] ,
        [   a owl:restriction ;
            owl:onProperty amsl:description ;
            owl:minCardinality "0"^^xsd:nonNegativeInteger ] ,
        [   a owl:restriction ;
            owl:onProperty amsl:digitallyCopy ;
            owl:maxCardinality "1"^^xsd:nonNegativeInteger ] ,
        [   a owl:restriction ;
            owl:onProperty amsl:erAltTitle ;
            owl:minCardinality "0"^^xsd:nonNegativeInteger ] ,
        [   a owl:restriction ;
            owl:onProperty amsl:erStatus ;
            owl:cardinality "1"^^xsd:nonNegativeInteger ] ,
        [   a owl:restriction ;
            owl:onProperty amsl:erType ;
            owl:cardinality "1"^^xsd:nonNegativeInteger ] ,
        [   a owl:restriction ;
            owl:onProperty amsl:file ;
            owl:minCardinality "0"^^xsd:nonNegativeInteger ] ,
        [   a owl:restriction ;
            owl:onProperty amsl:hasRemoteAccess ;
            owl:maxCardinality "1"^^xsd:nonNegativeInteger ] ,
        [   a owl:restriction ;
            owl:onProperty amsl:illNote ; # momentan nicht im Template
            owl:maxCardinality "1"^^xsd:nonNegativeInteger ] ,
        [   a owl:restriction ;
            owl:onProperty amsl:illset ; # momentan nicht im Template
            owl:maxCardinality "1"^^xsd:nonNegativeInteger ] ,
        [   a owl:restriction ;
            owl:onProperty amsl:illElectronic ; # momentan nicht im Template
            owl:maxCardinality "1"^^xsd:nonNegativeInteger ] ,
        [   a owl:restriction ;
            owl:onProperty amsl:illPrintOrFax ; # momentan nicht im Template
            owl:maxCardinality "1"^^xsd:nonNegativeInteger ] ,    
        [   a owl:restriction ;
            owl:onProperty amsl:individualContractItems ;
            owl:maxCardinality "1"^^xsd:nonNegativeInteger ] ,
        [   a owl:restriction ;
            owl:onProperty amsl:initialAcquisitionDate ;
            owl:maxCardinality "1"^^xsd:nonNegativeInteger ] ,
        [   a owl:restriction ;
            owl:onProperty amsl:internalContact ;
            owl:minCardinality "0"^^xsd:nonNegativeInteger ] ,
        [   a owl:restriction ;
            owl:onProperty amsl:licensee ;
            owl:cardinality "1"^^xsd:nonNegativeInteger ] ,
        [   a owl:restriction ;
            owl:onProperty amsl:licensingNote ;
            owl:minCardinality "0"^^xsd:nonNegativeInteger  ] ,
        [   a owl:restriction ;
            owl:onProperty amsl:licensor ;
            owl:cardinality "1"^^xsd:nonNegativeInteger ] ,
        [   a owl:restriction ;
            owl:onProperty amsl:linkToDescription ;
            owl:minCardinality "0"^^xsd:nonNegativeInteger ] ,
        [   a owl:restriction ;
            owl:onProperty amsl:localSystemNumber ;
            owl:minCardinality "0"^^xsd:nonNegativeInteger ] ,
        [   a owl:restriction ;
            owl:onProperty amsl:mailFile ;
            owl:minCardinality "0"^^xsd:nonNegativeInteger ] ,
        [   a owl:restriction ;
            owl:onProperty amsl:pCopy ;
            owl:maxCardinality "1"^^xsd:nonNegativeInteger ] ,
        [   a owl:restriction ;
            owl:onProperty amsl:platform ;
            owl:minCardinality "1"^^xsd:nonNegativeInteger ] ,
        [   a owl:restriction ;
            owl:onProperty amsl:previousContract ;
            owl:maxCardinality "1"^^xsd:nonNegativeInteger ] ,
        [   a owl:restriction ;
            owl:onProperty amsl:primaryAccessURI ; # momentan nicht im Template
            owl:maxCardinality "1"^^xsd:nonNegativeInteger ] ,
        [   a owl:restriction ;
            owl:onProperty amsl:scholarlySharing ;
            owl:maxCardinality "1"^^xsd:nonNegativeInteger ] ,
        [   a owl:restriction ;
            owl:onProperty amsl:shutDownDate ;
            owl:maxCardinality "1"^^xsd:nonNegativeInteger ] ,
        [   a owl:restriction ;
            owl:onProperty amsl:terminationDate ;
            owl:maxCardinality "1"^^xsd:nonNegativeInteger ] ,
        [   a owl:restriction ;
            owl:onProperty amsl:terminationReason ;
            owl:minCardinality "0"^^xsd:nonNegativeInteger ] ,
        [   a owl:restriction ;
            owl:onProperty dct:creator ;
            owl:maxCardinality "1"^^xsd:nonNegativeInteger ] ,
        [   a owl:restriction ;
            owl:onProperty rdfs:comment ;
            owl:minCardinality "0"^^xsd:nonNegativeInteger ] ,
        [   a owl:restriction ;
            owl:onProperty rdfs:label ;
            owl:minCardinality "1"^^xsd:nonNegativeInteger ] ;
    rdfs:comment "Ein Geschäftsvertrag zwischen der Bibliothek und weiteren Parteien. Dieser Vertragsteil beinhaltet die Basisinformationen (statische Daten) eines Vertrages."@de ,
        "A class modeling a business contract between the library and one or more parties. This one contains the basic (static) properties of a contract."@en ;
    rdfs:seeAlso "ERMI terms: _Acquisition Entity_ (cf. https://old.diglib.org/pubs/dlf102/ERMFINAL.pdf, p. 141)" ;
    rdfs:seeAlso "ERMI terms: _License Entity_ (cf. https://old.diglib.org/pubs/dlf102/ERMFINAL.pdf, p. 144)" .

amsl:BranchOffice a owl:Class ;
    rdfs:label "Branch Office"@en ,
        "Zweigstelle"@de ;
    rdfs:subClassOf 
        [   a owl:restriction ;
            owl:onProperty amsl:orgNote ;
            owl:minCardinality "0"^^xsd:nonNegativeInteger ] ,
        [   a owl:restriction ;
            owl:onProperty rdfs:comment  ;
            owl:minCardinality "0"^^xsd:nonNegativeInteger ] ,
        [   a owl:restriction ;
            owl:onProperty rdfs:label  ;
            owl:minCardinality "1"^^xsd:nonNegativeInteger ] ,
        [   a owl:restriction ;
            owl:onProperty skos:altLabel   ;
            owl:minCardinality "0"^^xsd:nonNegativeInteger ] ,
        [   a owl:restriction ;
            owl:onProperty vcard:country-name ;
            owl:maxCardinality "1"^^xsd:nonNegativeInteger ] ,
        [   a owl:restriction ;
            owl:onProperty vcard:hasEmail  ;
            owl:minCardinality "0"^^xsd:nonNegativeInteger ] ,
        [   a owl:restriction ;
            owl:onProperty vcard:hasTelephone ;
            owl:minCardinality "0"^^xsd:nonNegativeInteger ] ,
        [   a owl:restriction ;
            owl:onProperty vcard:hasURL  ;
            owl:minCardinality "0"^^xsd:nonNegativeInteger ] ,
        [   a owl:restriction ;
            owl:onProperty vcard:locality  ;
            owl:maxCardinality "1"^^xsd:nonNegativeInteger ] ,
        [   a owl:restriction ;
            owl:onProperty vcard:postal-code ;
            owl:maxCardinality "1"^^xsd:nonNegativeInteger ] ,
        [   a owl:restriction ;
            owl:onProperty vcard:street-address  ;
            owl:maxCardinality "1"^^xsd:nonNegativeInteger ] ;
    rdfs:comment "Eine Zweigstelle einer Organisation."@de ,
        "A branch office of an organisation."@en .

amsl:Budget a owl:Class ;
    rdfs:label "Budget"@de ,
        "Budget"@en ;
    rdfs:subClassOf 
        [   a owl:restriction ;
            owl:onProperty amsl:budgetAbbr  ;
            owl:maxCardinality "1"^^xsd:nonNegativeInteger ] ,
        [   a owl:restriction ;
            owl:onProperty rdfs:comment ;
            owl:minCardinality "0"^^xsd:nonNegativeInteger ] ,
        [   a owl:restriction ;
            owl:onProperty rdfs:label  ;
            owl:minCardinality "1"^^xsd:nonNegativeInteger ] ;
    rdfs:comment "Budgets für die Medienerwerbung."@de ,
    	 "Budgets for media acquisition."@en .

amsl:Collection a owl:Class ;
    rdfs:label "Kollektion"@de , 
        "Collection"@en ;
    rdfs:comment "Eine Kollektion oder Sammlung, die nicht näher bestimmte zusammengehörige Daten umfasst. Detailliertere Beschreibungen sind über Unterklassen möglich."@de , 
        "A collection containing not further specified data. Subclasses are available or a more detailed description."@en .

amsl:ContractData a owl:Class ;
    rdfs:label "Vertragsdaten"@de ,
        "ContractData"@en ;
    rdfs:comment "Ein Geschäftsvertrag zwischen üblicherweise der Bibliothek und einer anderen Partei. Instanzen werden im Allgemeinen nur von den Unterklassen gebildet."@de ,
        "A business contract between usually the library and another party. Generally, only the subclasses are instanciated."@en .

amsl:ContractItem a owl:Class ;
    rdfs:label "Vertragsposition"@de ,
        "Contract Item"@en ;
    rdfs:subClassOf 
        [   a owl:restriction ;
            owl:onProperty amsl:contractItemOf  ;
            owl:cardinality "1"^^xsd:nonNegativeInteger ] ,
        [   a owl:restriction ;
            owl:onProperty amsl:coverageDepth  ;
            owl:maxCardinality "1"^^xsd:nonNegativeInteger ] ,
        [   a owl:restriction ;
            owl:onProperty amsl:coverageNotes  ;
            owl:maxCardinality "1"^^xsd:nonNegativeInteger ] ,
        [   a owl:restriction ;
            owl:onProperty amsl:dateFirstIssueOnline  ;
            owl:maxCardinality "1"^^xsd:nonNegativeInteger ] ,
        [   a owl:restriction ;
            owl:onProperty amsl:dateLastIssueOnline  ;
            owl:maxCardinality "1"^^xsd:nonNegativeInteger ] ,
        [   a owl:restriction ;
            owl:onProperty amsl:doi  ;
            owl:minCardinality "0"^^xsd:nonNegativeInteger ] ,
        [   a owl:restriction ;
            owl:onProperty amsl:eisbn  ;
            owl:minCardinality "0"^^xsd:nonNegativeInteger ] ,
        [   a owl:restriction ;
            owl:onProperty amsl:eissn  ;
            owl:minCardinality "0"^^xsd:nonNegativeInteger ] ,
        [   a owl:restriction ;
            owl:onProperty amsl:embargoInfo  ;
            owl:maxCardinality "1"^^xsd:nonNegativeInteger ] ,
        [   a owl:restriction ;
            owl:onProperty amsl:itemPrice  ;
            owl:maxCardinality "1"^^xsd:nonNegativeInteger ] ,
        [   a owl:restriction ;
            owl:onProperty amsl:localSystemNumber  ;
            owl:minCardinality "0"^^xsd:nonNegativeInteger ] ,
        [   a owl:restriction ;
            owl:onProperty amsl:numberFirstIssueOnline  ;
            owl:maxCardinality "1"^^xsd:nonNegativeInteger ] ,
        [   a owl:restriction ;
            owl:onProperty amsl:numberFirstVolumeOnline  ;
            owl:maxCardinality "1"^^xsd:nonNegativeInteger ] ,
        [   a owl:restriction ;
            owl:onProperty amsl:numberLastIssueOnline  ;
            owl:maxCardinality "1"^^xsd:nonNegativeInteger ] ,
        [   a owl:restriction ;
            owl:onProperty amsl:numberLastVolumeOnline  ;
            owl:maxCardinality "1"^^xsd:nonNegativeInteger ] ,
        [   a owl:restriction ;
            owl:onProperty amsl:pisbn  ;
            owl:minCardinality "0"^^xsd:nonNegativeInteger ] ,
        [   a owl:restriction ;
            owl:onProperty amsl:pissn  ;
            owl:minCardinality "0"^^xsd:nonNegativeInteger ] ,
        [   a owl:restriction ;
            owl:onProperty amsl:primaryAccessURI  ;
            owl:maxCardinality "1"^^xsd:nonNegativeInteger ] ,
        [   a owl:restriction ;
            owl:onProperty amsl:proprietaryID  ;
            owl:maxCardinality "1"^^xsd:nonNegativeInteger ] ,
        [   a owl:restriction ;
            owl:onProperty bibo:issn ;
            owl:minCardinality "0"^^xsd:nonNegativeInteger ] ,
        [   a owl:restriction ;
            owl:onProperty bibo:shortTitle  ;
            owl:minCardinality "0"^^xsd:nonNegativeInteger ] ,
        [   a owl:restriction ;
            owl:onProperty count:hasItemDatatype   ;
            owl:maxCardinality "1"^^xsd:nonNegativeInteger ] ,
        [   a owl:restriction ;
            owl:onProperty count:hasPerformance   ;
            owl:minCardinality "0"^^xsd:nonNegativeInteger ] ,
        [   a owl:restriction ;
            owl:onProperty count:isAccessibleVia ;
            owl:maxCardinality "1"^^xsd:nonNegativeInteger ] ,
        [   a owl:restriction ;
            owl:onProperty count:isContainedIn   ;
            owl:minCardinality "0"^^xsd:nonNegativeInteger ] ,
        [   a owl:restriction ;
            owl:onProperty dc:creator   ;
            owl:minCardinality "0"^^xsd:nonNegativeInteger ] ,
        [   a owl:restriction ;
            owl:onProperty dc:publisher  ;
            owl:minCardinality "0"^^xsd:nonNegativeInteger ] ,
        [   a owl:restriction ;
            owl:onProperty dc:title ;
            owl:minCardinality "0"^^xsd:nonNegativeInteger ] ,
        [   a owl:restriction ;
            owl:onProperty dct:issued  ;
            owl:mainCardinality "0"^^xsd:nonNegativeInteger ] ,
        [   a owl:restriction ;
            owl:onProperty dct:language  ;
            owl:maxCardinality "1"^^xsd:nonNegativeInteger ] ,
        [   a owl:restriction ;
            owl:onProperty rdfs:comment   ;
            owl:minCardinality "0"^^xsd:nonNegativeInteger ] ;
    rdfs:comment "Die einzelnen elektronischen Ressourcen, die von einem Vetrag oder einem Lizenzpaket umfasst werden."@de ,
    	"Individual electronic resources that are contained in a license contract or package."@en .

amsl:FacultyShare a owl:Class ;
    rdfs:label "Fakultätsanteil"@de ,
        "Faculty share"@en ;
    rdfs:subClassOf
        [   a owl:restriction ;
            owl:onProperty amsl:faculty   ;
            owl:cardinality "1"^^xsd:nonNegativeInteger ] ,
        [   a owl:restriction ;
            owl:onProperty amsl:percentage  ;
            owl:cardinality "1"^^xsd:nonNegativeInteger ] ,
        [   a owl:restriction ;
            owl:onProperty rdfs:comment   ;
            owl:minCardinality "0"^^xsd:nonNegativeInteger ] ,
        [   a owl:restriction ;
            owl:onProperty rdfs:label   ;
            owl:minCardinality "1"^^xsd:nonNegativeInteger ] ;
    rdfs:comment "Der Anteil an einem Vertrag, den eine bestimmte Fakultät trägt."@de ,
        "The share of a license contract a certain faculty bears."@en .

amsl:MetadataCollection a owl:Class ;
    rdfs:subClassOf amsl:Collection ;
    rdfs:label "Metadatenkollektion"@de ,
        "Metadata Collection"@en ;
    rdfs:subClassOf 
        [   a owl:restriction ;
            owl:onProperty amsl:collectionID  ;
            owl:maxCardinality "1"^^xsd:nonNegativeInteger ] ,
        [   a owl:restriction ;
            owl:onProperty amsl:contentFile ;
            owl:minCardinality "0"^^xsd:nonNegativeInteger ] ,
        [   a owl:restriction ;
            owl:onProperty amsl:coveredMediumID  ;
            owl:minCardinality "0"^^xsd:nonNegativeInteger ] ,
        [   a owl:restriction ;
            owl:onProperty amsl:evaluateHoldingsFileFor ;
            owl:minCardinality "0"^^xsd:nonNegativeInteger ] ,
        [   a owl:restriction ;
            owl:onProperty amsl:includedInMetadataSource  ;
            owl:cardinality "1"^^xsd:nonNegativeInteger ] ,
        [   a owl:restriction ;
            owl:onProperty amsl:linkToContentFile ;
            owl:minCardinality "0"^^xsd:nonNegativeInteger ] ,
        [   a owl:restriction ;
            owl:onProperty amsl:metadataUsagePermittedForLibrary ;
            owl:minCardinality "0"^^xsd:nonNegativeInteger ] ,
        [   a owl:restriction ;
            owl:onProperty amsl:metadataUsageRestricted ;
            owl:cardinality "1"^^xsd:nonNegativeInteger ] ,
        [   a owl:restriction ;
            owl:onProperty  amsl:metadataUsedByLibrary  ;
            owl:minCardinality "0"^^xsd:nonNegativeInteger ] ,
        [   a owl:restriction ;
            owl:onProperty amsl:productISIL ;
            owl:maxCardinality "1"^^xsd:nonNegativeInteger ] ,
        [   a owl:restriction ;
            owl:onProperty amsl:ticketURL  ;
            owl:minCardinality "0"^^xsd:nonNegativeInteger ] ,
        [   a owl:restriction ;
            owl:onProperty rdfs:comment ;
            owl:minCardinality "0"^^xsd:nonNegativeInteger ] ,
        [   a owl:restriction ;
            owl:onProperty rdfs:label  ;
            owl:minCardinality "1"^^xsd:nonNegativeInteger ] ;
    rdfs:comment "Eine Kollektion von Metadaten, die bspw. in einen Bibliothekskatalog eingespielt wird."@de ,
        "A collection of metadata that is to be integrated in e.g. a library catalog."@en .

amsl:MetadataSource a owl:Class;
    rdfs:subClassOf amsl:Source ;
    rdfs:label "Metadatenquelle"@de ,
        "Metadata Source"@en ;
    rdfs:subClassOf
        [   a owl:restriction ;
            owl:onProperty  amsl:deduplicationInferiorTo  ;
            owl:minCardinality "0"^^xsd:nonNegativeInteger ] ,
        [   a owl:restriction ;
            owl:onProperty  amsl:externalContact  ;
            owl:minCardinality "0"^^xsd:nonNegativeInteger ] ,
        [   a owl:restriction ;
            owl:onProperty  amsl:indexingLevel  ;
            owl:maxCardinality "1"^^xsd:nonNegativeInteger ] ,
        [   a owl:restriction ;
            owl:onProperty  amsl:internalContact  ;
            owl:minCardinality "0"^^xsd:nonNegativeInteger ] ,
        [   a owl:restriction ;
            owl:onProperty amsl:licensingNote ;
            owl:minCardinality "0"^^xsd:nonNegativeInteger ] ,
        [   a owl:restriction ;
            owl:onProperty amsl:linkToContract  ;
            owl:minCardinality "0"^^xsd:nonNegativeInteger ] ,
        [   a owl:restriction ;
            owl:onProperty amsl:metadataSourceImplStatus  ;
            owl:cardinality "1"^^xsd:nonNegativeInteger ] ,
        [   a owl:restriction ;
            owl:onProperty amsl:nextUpdateDate  ;
            owl:maxCardinality "1"^^xsd:nonNegativeInteger ] ,
        [   a owl:restriction ;
            owl:onProperty amsl:primaryAccessURI  ;
            owl:maxCardinality "1"^^xsd:nonNegativeInteger ] ,
        [   a owl:restriction ;
            owl:onProperty amsl:solrShard  ;
            owl:maxCardinality "1"^^xsd:nonNegativeInteger ] ,
        [   a owl:restriction ;
            owl:onProperty amsl:sourceID  ;
            owl:cardinality "1"^^xsd:nonNegativeInteger ] ,
        [   a owl:restriction ;
            owl:onProperty amsl:ticketURL  ;
            owl:minCardinality "0"^^xsd:nonNegativeInteger ] ,
        [   a owl:restriction ;
            owl:onProperty amsl:updateRhythm  ;
            owl:maxCardinality "1"^^xsd:nonNegativeInteger ] ,
        [   a owl:restriction ;
            owl:onProperty dct:creator  ;
            owl:minCardinality "0"^^xsd:nonNegativeInteger ] ,
        [   a owl:restriction ;
            owl:onProperty dct:format   ;
            owl:maxCardinality "1"^^xsd:nonNegativeInteger ] ,
        [   a owl:restriction ;
            owl:onProperty gr:availableDeliveryMethods  ;
            owl:minCardinality "0"^^xsd:nonNegativeInteger ] ,
       [   a owl:restriction ;
            owl:onProperty rdfs:comment ;
            owl:minCardinality "0"^^xsd:nonNegativeInteger ] ,
        [   a owl:restriction ;
            owl:onProperty rdfs:label  ;
            owl:minCardinality "1"^^xsd:nonNegativeInteger ] ;
    rdfs:comment "Eine Quelle, die (bibliographische) Metadaten anbietet."@de ,
        "A source providing (bibliographic) metadata"@en .

amsl:LicensePackage a owl:Class ;
    rdfs:label "Paket"@de ,
        "License Package"@en ;
    owl:rdfs:subClassOf
        [   a owl:restriction ;
            owl:onProperty amsl:contractContainingPackage  ;
            owl:cardinality "1"^^xsd:nonNegativeInteger ] ,
        [   a owl:restriction ;
            owl:onProperty amsl:ezbAnchor  ;
            owl:maxCardinality "1"^^xsd:nonNegativeInteger ] ,
        [   a owl:restriction ;
            owl:onProperty amsl:contentFile  ;
            owl:minCardinality "0"^^xsd:nonNegativeInteger ] ,
        [   a owl:restriction ;
            owl:onProperty amsl:linkToContentFile  ;
            owl:minCardinality "0"^^xsd:nonNegativeInteger ] ,
        [   a owl:restriction ;
            owl:onProperty amsl:productISIL   ;
            owl:maxCardinality "1"^^xsd:nonNegativeInteger ] ,
        [   a owl:restriction ;
            owl:onProperty rdfs:comment ;
            owl:minCardinality "0"^^xsd:nonNegativeInteger ] ,
        [   a owl:restriction ;
            owl:onProperty rdfs:label  ;
            owl:minCardinality "1"^^xsd:nonNegativeInteger ] ;
    rdfs:comment "Ein Lizenzvertrag kann aus mehreren Lizenzpaketen zusammengestellt sein."@de ,
        "A license contract can be made up by several license packages."@en .


amsl:Platform a owl:Class ;
    rdfs:label "Plattform"@de ,
        "Platform"@en ;
    owl:rdfs:subClassOf
        [   a owl:restriction ;
            owl:onProperty amsl:shibbolethImplStatus  ;
            owl:maxCardinality "1"^^xsd:nonNegativeInteger ] ,
        [   a owl:restriction ;
            owl:onProperty rdfs:comment ;
            owl:minCardinality "0"^^xsd:nonNegativeInteger ] ,
        [   a owl:restriction ;
            owl:onProperty rdfs:label  ;
            owl:minCardinality "1"^^xsd:nonNegativeInteger ] ,
        [   a owl:restriction ;
            owl:onProperty vcard:hasURL    ;
            owl:maxCardinality "1"^^xsd:nonNegativeInteger ] ;
    rdfs:comment "Das Portal bzw. der Service, der die Inhalte bereitstellt und zugänglich macht."@de ,
        "The portal resp. service providing the electronic content and the access to it."@en ;
        rdfs:seeAlso "ERMI terms: _Interface Entity_ (cf. https://old.diglib.org/pubs/dlf102/ERMFINAL.pdf, p. 139)" .


amsl:Source a owl:Class ;
    rdfs:label "Quelle"@de , 
        "Source"@en ;
    rdfs:comment "Eine Quelle, die nicht näher bestimmte Daten anbietet. Detailliertere Beschreibungen sind über Unterklassen möglich."@de , 
        "A source providing not further specified data. Subclasses are available or a more detailed description."@en .


amsl:Subtotal a owl:Class ;
    rdfs:label "Teilsumme"@de ,
        "Subtotal"@en ;
    owl:rdfs:subClassOf
        [   a owl:restriction ;
            owl:onProperty amsl:annualBudget  ;
            owl:maxCardinality "1"^^xsd:nonNegativeInteger ] ,
        #  amsl:budget 
        [   a owl:restriction ;
            owl:onProperty amsl:expectedPrice  ;
            owl:maxCardinality "1"^^xsd:nonNegativeInteger ] ,
        [   a owl:restriction ;
            owl:onProperty amsl:invoicePriceGrossEUR  ;
            owl:maxCardinality "1"^^xsd:nonNegativeInteger ] ,
        [   a owl:restriction ;
            owl:onProperty amsl:invoicePriceGrossGBP  ;
            owl:maxCardinality "1"^^xsd:nonNegativeInteger ] ,
        [   a owl:restriction ;
            owl:onProperty amsl:invoicePriceGrossUSD  ;
            owl:maxCardinality "1"^^xsd:nonNegativeInteger ] ,
        [   a owl:restriction ;
            owl:onProperty amsl:invoicePriceNetEUR  ;
            owl:maxCardinality "1"^^xsd:nonNegativeInteger ] ,
        [   a owl:restriction ;
            owl:onProperty amsl:invoicePriceNetGBP  ;
            owl:maxCardinality "1"^^xsd:nonNegativeInteger ] ,
        [   a owl:restriction ;
            owl:onProperty amsl:invoicePriceNetUSD  ;
            owl:maxCardinality "1"^^xsd:nonNegativeInteger ] ,
        [   a owl:restriction ;
            owl:onProperty rdfs:comment ;
            owl:minCardinality "0"^^xsd:nonNegativeInteger ] ,
        [   a owl:restriction ;
            owl:onProperty rdfs:label  ;
            owl:minCardinality "1"^^xsd:nonNegativeInteger ] ;
    rdfs:comment "Eine Teilsumme bspw. eines Rechnungs- oder Planpreises."@de ,
        "A subtotal of e.g. an invoice or expected price." .

  



######################## Properties #####################################

amsl:acqMethod a owl:ObjectProperty ;
    rdfs:label "Erwerbungsart"@de ,
        "acquisition method"@en ;
    rdfs:comment "Verknüpft die Art, auf die in einem Vertrages beinhalteten Lizenzen erworben wurden."@de ,
    	"Links the method of acquisition used to purchase the licenses of a contract."@en ;
    rdfs:domain amsl:BasicContractData ;  
    rdfs:range amsl:AcqNote .

amsl:annualBudget a owl:ObjectProperty ;
    rdfs:label "Jahresbudget"@de ,
        "annual budget"@en ;
    rdfs:comment "Verknüpft das Jahresbudget, aus dem ein Betrag finanziert wird."@de ,
        "Links the annual budget a sum is financed from."@en ;
    rdfs:domain amsl:AnnualContractData ;
    rdfs:range amsl:AnnualBudget .    

amsl:annualPrice a owl:DatatypeProperty ;
    rdfs:label "Jahrespreis (EUR)"@de ,
        "annual price (EUR)"@en ;
    rdfs:comment "Verknüpft den jährlichen Preis eines Lizenzvertrages in Euro."@de ,
        "Links the annual price of a license contract in euro."@en ;
    rdfs:domain amsl:AnnualContractData ;
    rdfs:range xsd:decimal .

amsl:archivedAnnualContractDataLabel a owl:DatatypeProperty ;
    rdfs:label "Archivierte Vertragsjahresdaten"@de ,
        "archived annual contract data"@en ;
    rdfs:comment "Verknüpft Vertragsbasisdaten mit dem Label solcher Vertragsjahresdaten, die im Zuge einer Archivierungsfunktion nicht mehr im aktuellen Datenbestand verfügbar ist. Auf diese Weise ist im aktuellen Datenbestand immer noch eine Historie sichtbar."@de ,
        "Links basic contract data with the label of annual contract data that are no longer available in the current data set, due to an archiving functionality. This way the current data set does still provide a history of annual contract data."@en ;
    rdfs:domain amsl:BasicContractData .

amsl:archivingNote a owl:DataTypeProperty ;
    rdfs:label "Verfügbarkeit nach Vertragsende"@de ,
        "availability after termination"@en ;
    rdfs:comment "Verknüpft Informationen zur Verfügbarkeite der elektronischen Ressourcen nach Vertragsende (Archivrecht, Format...)."@de ,
         "Links additional information related to archiving rights, product, and format."@en ;
    rdfs:seeAlso "ERMI terms: _Archiving Note_ (cf. https://old.diglib.org/pubs/dlf102/ERMFINAL.pdf, p. 159)" ; 
    rdfs:domain amsl:BasicContractData .     

amsl:authMethod a owl:ObjectProperty ;
    rdfs:label "Authentifizierungsmethode"@de ,
        "authentication method"@en ;
    rdfs:comment "Verknüpft die nötige Authentifizierungsmethode, um Zugang zu den lizenzierten elektronischen Ressourcen zu erhalten."@de ,
    	"Links the method of authentification required to gain access to the licensed electronic resources."@en ;        
    rdfs:domain amsl:BasicContractData ;
    rdfs:range amsl:AuthMethod .

amsl:authorizedUser a owl:ObjectProperty ;
    rdfs:label "Autorisierte Nutzer"@de ,
        "authorized users"@en ;
    rdfs:comment "Verknüpft eine oder mehrere Nutzergruppen, die für zur Nutzung der lizenzierten elektronischen Ressourcen autorisiert sind."@de ,
        "Links one or several usersgroups that are authorized to use the licensed electronic resources."@en ;
    rdfs:seeAlso "ERMI terms: _Authorized User Definition_ (cf. https://old.diglib.org/pubs/dlf102/ERMFINAL.pdf, p. 151)" ; 
    rdfs:domain amsl:BasicContractData ;
    rdfs:range amsl:UserGroup .

amsl:balanceFile a owl:ObjectProperty ;
    rdfs:subPropertyOf amsl:file ;
    rdfs:label "Über-/Fehlbertragsdatei"@de ,
        "balance file"@en ;
    rdfs:comment "Verknüpft eine Ressource des Typs Dokument, die eine Über-/Fehlbetragsrechnungsdatei beschreibt."@de , 
        "Links a resource of the type Document describing a balance file."@en   ;
    rdfs:domain amsl:AnnualContractData ;
    rdfs:range foaf:Document .    

amsl:basicContractData a owl:ObjectProperty ;
    rdfs:label "Zugehörige Vertragsbasisdaten"@de ,
        "associated basic contract data"@en ;
    rdfs:comment "Vernüpft die übergeordnteten Vertragsbasisdaten, zu denen bestimmte Vertragsjahresdaten gehören."@de ,
        "Links the superordinated basic contract data, certain annual contract data are associated with."@en ;
    rdfs:domain amsl:AnnualContractData ;
    rdfs:range amsl:BasicContractData .

amsl:branchOffice a owl:ObjectProperty ;
    rdfs:label "Zweigstelle"@de ,
        "branch office"@en ;
    rdfs:comment "Verknüpft ine Zweigstelle einer Organisation."@de ,
        "Links a branch office of an organisation."@en ;
    rdfs:domain foaf:Organization ;
    rdfs:range amsl:BranchOffice .

amsl:budget a owl:ObjectProperty ;
    rdfs:label "Budget"@de ,
        "budget"@en ;
    rdf:comment "Verknüpft das Budget, das mit den Kosten für einen Lizenzvertrag belastet wird."@de ,
    	"Links the budget charged with the costs of a license contract."@en ;
    rdfs:domain  [ a owl:Class ;
        owl:unionOf ( amsl:AnnualBudget amsl:Subtotal ) ] ;
    rdfs:range amsl:Budget .

amsl:budgetAbbr a owl:DataTypeProperty ;
    rdfs:label "Budgetkürzel"@de ,
        "budget abbreviation"@en ;
    rdfs:comment "Verknüpft die intern gebräuchliche Abkürzung eines Budets."@de ,
        "Links the internally common abbreviation of a budget name."@en ;
    rdfs:domain amsl:Budget .

amsl:collectionID a owl:DatatypeProperty ;
    rdfs:label "Collection ID"@de ,
        "collection ID"@en ;
    rdfs:comment "Verknüpft die Collection ID einer Metadatenkollektion"@de ,
        "Links the collection ID of a metadata collection"@en ;
    rdfs:domain amsl:Collection .    

amsl:concUser a owl:DatatypeProperty ;
    rdfs:label "Parallelzugriffe"@de ,
        "concurrent users"@en ;
    rdfs:comment "Verknüpft die Anzahl der in den Lizenzbedingungen eines Vertrages angegeben Parallelzugriffe auf eine elektronische Ressource."@de ,
        "Links the number of concurrent users for an electronic resource licensed in a contract."@en ;
    rdfs:seeAlso "ERMI terms: _Concurrent User_ (cf. https://old.diglib.org/pubs/dlf102/ERMFINAL.pdf, p. 157)" ; 
    rdfs:domain amsl:BasicContractData .

amsl:consortium a owl:ObjectProperty ;
    rdfs:label "Konsortium"@de ,
        "consortium"@en ;
    rdfs:comment "Verknüpft ein beteiligtes Bibliothekskonsortium (Zusammenschluss von Bibliotheken)"@de ,
    	"Links an involved library consortium (association of libraries)"@en ;
    rdfs:domain amsl:BasicContractData ;
    rdfs:range foaf:Organization .

amsl:consortiumLeader a owl:ObjectProperty ;
    rdfs:label "Konsortialführer"@de ,
        "consortium leader"@en ;
    rdfs:comment "Verknüpft die Organisation, die für einen bestimmten konsortialen Lizenzvertrag die Rolle des Konsortialführers innehat."@de ,
        "Links the organization operating as consortium leader for a certain consortial license contract."@en ;
    rdfs:domain amsl:BasicContractData ;
    rdfs:range foaf:Organization .

amsl:contactNote a owl:DatatypeProperty ;
    rdfs:label "Notiz zum Kontakt"@de ,
        "contact note"@en ;
    rdfs:comment "Verknüft weitere notierte Details zu einem Kontakt."@de ,
        "Links further listed details on a contact."@en ;
    rdfs:domain foaf:Person .

amsl:contentFile a owl:ObjectProperty ;
    rdfs:subPropertyOf amsl:file ;
    rdfs:label "Content-File"@de ,
        "content file"@en ;
    rdfs:comment "Verknüpft eine Ressource des Typs Dokument, die ein Content-File darstellt."@de , 
        "Links a resource of the type Document."@en   ;
    rdfs:domain [ a owl:Class ;
        owl:unionOf ( amsl:MetadataCollection amsl:LicensePackage ) ] ;
    rdfs:range foaf:Document .  

amsl:contractContainingPackage a owl:ObjectProperty ;
    rdfs:label "dieses Paket umfassender Vertrag"@de ,
        "contract containing this package"@en ;
    rdfs:comment "Verknüpft die Vertragsjahresdaten, zu denen ein bestimmtes Lizenzpaket gehört."@de ,
        "Links the the annual contact data a certain license package is associated with."@en ;        
    rdfs:domain amsl:LicensePackage ;
    rdfs:range amsl:AnnualContractData .

amsl:contractFile a owl:ObjectProperty ;
    rdfs:subPropertyOf amsl:file ;
    rdfs:label "Vertragsdatei"@de ,
     "contract file"@en ;
    rdfs:comment "Verknüpft eine Ressource des Typs Dokument, die eine Vertragsdatei beschreibt."@de , 
        "Links a resource of the type Document, describing a contract file."@en   ;
    rdfs:seeAlso "ERMI terms: _License Uniform Resource Identifier_ (cf. https://old.diglib.org/pubs/dlf102/ERMFINAL.pdf, p. 145)" ; 
    rdfs:domain [ a owl:Class ;
        owl:unionOf ( amsl:BasicContractData amsl:AnnualContractData ) ] ;
    rdfs:range foaf:Document .

amsl:contractItemOf a owl:ObjectProperty ;
    rdfs:label "Vertragsposition von"@de ,
        "contract item of"@en ;
    rdfs:comment "Verknüpft eine bestimmte Vertragsposition mit dem Lizenzpaket, in dem sie enthalten ist."@de ,
        "Links a certain contract item with the license package it is contained in."@en ;
    rdfs:range  amsl:LicensePackage ;
    rdfs:domain amsl:ContractItem  .

amsl:costCenter a owl:DataTypeProperty ;
    rdfs:label "Kostenstelle"@de ,
        "cost center"@en ;
    rdfs:comment "Verknüpft eine Kostenstelle. Sie ist ein Kostenrechnungsobjekt mit der Aufgabe, die in einem Unternehmensteil, meist einer Abteilung, angefallenen Kosten zu sammeln."@de ,
        "Links a cost center. It is part of an organization that does not produce direct profit and adds to the cost of running a company."@en ;
    rdfs:domain aiiso:Faculty .

amsl:coursePackE a owl:ObjectProperty ;
    rdfs:label "Reader elektronisch"@de ,
        "course pack electronic"@en ;
    rdfs:comment "Verknüpft Infomationen über das Recht eines Fakultätsmitgliedes, lizenziertes Material in Zusammnenstellungen in elektronischer Form für Studentengruppen zu Anleitungszwecken zu verwenden."@de ,
        "Links information on the right to use licensed materials in collections or compilations of materials assembled in an electronic format by faculty members for use by students in a class for purposes of instruction."@en ;
    rdfs:seeAlso "ERMI terms: _Course Pack Electronic_ (cf. https://old.diglib.org/pubs/dlf102/ERMFINAL.pdf, p. 157)" ; 
    rdfs:domain amsl:BasicContractData ;
    rdfs:range amsl:LicenseTerm .

amsl:coursePackP a owl:ObjectProperty ;
    rdfs:label "Reader print"@de ,
        "course pack print"@en ;
    rdfs:comment "Verknüpft Infomationen über das Recht eines Fakultätsmitgliedes lizenziertes Material in Zusammnenstellungen in gedruckter Form für Studentengruppen zu Anleitungszwecken zu verwenden."@de ,
        "Links information on the right to use licensed materials in collections or compilations of materials assembled in a print format by faculty members for use by students in a class for purposes of instruction."@en ;
    rdfs:seeAlso "ERMI terms: _Course Pack Print_ (cf. https://old.diglib.org/pubs/dlf102/ERMFINAL.pdf, p. 156)" ; 
    rdfs:domain amsl:BasicContractData ;
    rdfs:range amsl:LicenseTerm .

amsl:courseReserveE a owl:ObjectProperty ;
    rdfs:label "Semesterapparat elektronisch"@de ,
        "course reserve electronic"@en ;
    rdfs:comment "Verknüpft Infomationen über das Recht digitale Kopien des lizenzierten Materials zu erstellen und sie in einem sicheren Netzwerk bereitzustellen."@de ,
        "Links information on the right to make electronic copies of the licensed materials and store them on a secure network."@en ;
    rdfs:seeAlso "ERMI terms: _Course Reserve Electronic_ (cf. https://old.diglib.org/pubs/dlf102/ERMFINAL.pdf, p. 156)" ; 
    rdfs:domain amsl:BasicContractData ;
    rdfs:range amsl:LicenseTerm .

amsl:courseReserveP a owl:ObjectProperty ;
    rdfs:label "Semesterapparat print"@de ,
        "course reserve print"@en ;
    rdfs:comment "Verknüpft Infomationen über das Recht gedruckte Kopien des lizenzierten Materials zu erstellen und sie in einem kontrollierten Bereich bereitzustellen."@de ,
        "Links information on the right to make print copies of the licensed materials and place them in a controlled circulation area of the library for reserve reading in conjunction with specific courses of instruction."@en ;
    rdfs:seeAlso "ERMI terms: _Course Reserve Print_ (cf. https://old.diglib.org/pubs/dlf102/ERMFINAL.pdf, p. 155)" ; 
    rdfs:domain amsl:BasicContractData ;
    rdfs:range amsl:LicenseTerm .    

amsl:coverageDepth a owl:ObjectProperty ;
    rdfs:label "Abdeckungstiefe"@de ,
        "coverage Depth"@en ;
    rdfs:comment "Verknüpft Informationen über die Tiefe, in der der Inhalt abgedeckt wird."@de ,
        "Links information on the extent to which content is covered."@en ;
    rdfs:domain amsl:ContractItem ;
    rdfs:range amsl:CoverageDepth .

amsl:coverageNotes a owl:DatatypeProperty ;
    rdfs:label "Abdeckungsnotiz"@de ,
        "coverage Notes"@en ;
    rdfs:comment "Verknüpft weiterführende Informationen über die Abdeckungstiefe."@de ,
        "Links further information on the coverage depth."@en ;
    rdfs:domain amsl:ContractItem .  

amsl:coveredMediumID a owl:ObjectProperty ;
    rdfs:label "abgedeckte Medien (ID)"@de ,
        "covered media (ID)"@en ;
    rdfs:comment "Verknüpft von den Metadaten der Kollektion abgedeckte Medien über deren IDs (ISSN, ISBN etc.)."@de , 
    "Links media covered by the collection's metadata via their IDs (ISSN, ISBN etc.)."@en ;
    rdfs:domain amsl:MetadataCollection .    

amsl:dataAvailability a owl:DatatypeProperty ;
    rdfs:label "(Meta-)Datenverfügbarkeit"@de ,
        "(meta)data availability"@en ;
    rdfs:comment "Verknüpft Informationen über die Verfügbarkeit von Metadaten zu den lizenzierten elektronischen Ressourcen."@de ,
        "Links information on the availability of metadata for the licensed electronic resources."@en ;
    rdfs:domain amsl:BasicContractData .    

amsl:dateFirstIssueOnline a owl:DatatypeProperty ;
    rdfs:label "Datum erster online verfügbarer Ausgabe"@de ,
        "date of first issue available online"@en ;
    skos:prefLabel "Datum erste verf. Ausg."@de ,
        "date first issue avail."@en ;
    rdfs:comment "Verknüpft das Datum der ersten online verfügbaren Ausgabe eines E-Journals oder E-Books."@de ,
        "Links the date of the first issue of an e-journal or e-book available online."@en ;
    rdfs:domain amsl:ContractItem ;
    rdfs:range xsd:date .   

amsl:dateLastIssueOnline a owl:DatatypeProperty ;
    rdfs:label "Datum letzter online verfügbarer Ausgabe"@de ,
        "date of last issue available online"@en ;
    skos:prefLabel "Datum letzte verf. Ausg."@de ,
        "date last issue avail."@en ;
    rdfs:comment "Verknüpft das Datum der letzten online verfügbaren Ausgabe eines E-Journals oder E-Books."@de ,
        "Links the date of the last issue of an e-journal or e-book available online."@en ;
    rdfs:domain amsl:ContractItem ;
    rdfs:range xsd:date .   

amsl:dbType a owl:ObjectProperty ;
    rdfs:label "Datenbanktyp"@de ,
        "database type"@en ;
    rdfs:comment "Verknüpft den Typ einer Datenbank."@de ,
    	"Links the type of a database."@en ;    
    rdfs:domain amsl:BasicContractData ;    
    rdfs:range amsl:DBType .

amsl:deduplicationInferiorTo a owl:ObjectProperty ;
    rdfs:label "Untergeordnet unter (Deduplizierung)"@de ,
        "inferior to (deduplication)"@en ;
    rdfs:comment "Verknüpft eine Metadatenquelle, der die aktuelle Quelle bei einem Deduplizierungsvorgang untergeordnet ist. Das heißt, die Metadaten der verknüpften Quelle werden bevorzugt."@de ,
        "Links a metadata source the current source is inferior to during a dedupliation process. That is, the metadata of the linked source are treated with priortity."@en ;
    rdfs:domain amsl:MetadataSource ;
    rdfs:range amsl:MetadataSource .

amsl:description a owl:DatatypeProperty ;
    rdfs:label "Beschreibung"@de ,
        "description"@en ;
    rdfs:comment "Verknüpft die Beschreibung des Inhalts. Es können Links zu weiteren relevanten Dokumenten (z. B. Inhaltsverzeichnis) enthalten sein."@de ,
        "Links an account of the content of the resource. It may include pointers to other relevant objects (e.g., tables of contents)."@en ;
    rdfs:seeAlso "ERMI terms: _Description_ (cf. https://old.diglib.org/pubs/dlf102/ERMFINAL.pdf, p. 136)" ;
    rdfs:domain amsl:BasicContractData .    

amsl:digitallyCopy a owl:ObjectProperty ;
    rdfs:label "Kopie digital"@de ,
        "digital copy "@en ;
    rdfs:comment "Verknüpft Infomationen über das Recht des Lizenznehmers und autorisierter Nutzer, eine digitale Kopie zu erstellen."@de ,
        "Links information on the right of the licensee and authorized users to download and digitally copy a reasonable portion of the licensed materials."@en ;
    rdfs:seeAlso "ERMI terms: _Digitally Copy_ (cf. https://old.diglib.org/pubs/dlf102/ERMFINAL.pdf, p. 153)" ; 
    rdfs:domain amsl:BasicContractData ;
    rdfs:range amsl:LicenseTerm .

amsl:doi a owl:ObjectProperty ; 
    rdfs:label "DOI"@de ,
        "DOI"@en ;
    rdfs:comment "Verknüpft den DOI eines Mediums."@de ,
        "Links the DOI of a medium."@en ;
    rdfs:seeAlso "ERMI terms: _Digital Object Identifier_ (cf. https://old.diglib.org/pubs/dlf102/ERMFINAL.pdf, p. 133)" .

amsl:eisbn a owl:ObjectProperty ;
    rdfs:label "E-ISBN"@de ,
        "E-ISBN"@en ;
    rdfs:comment "Verknüpft die E-ISBN eines Mediums."@de ,
        "Links the E-ISBN of a medium."@en ;
    rdfs:seeAlso "ERMI terms: _Electronic International Standard Book Number_ (cf. https://old.diglib.org/pubs/dlf102/ERMFINAL.pdf, p. 133)" .

amsl:eissn a owl:ObjectProperty ;
    rdfs:label "E-ISSN"@de ,
        "E-ISSN"@en ;
    rdfs:comment "Verknüpft die E-ISSN eines Mediums."@de ,
        "Links the E-ISSN of a medium."@en ;
    rdfs:seeAlso "ERMI terms: _Electronic International Standard Serial Number_ (cf. https://old.diglib.org/pubs/dlf102/ERMFINAL.pdf, p. 133)" .

amsl:embargoInfo a owl:DatatypeProperty ;
    rdfs:label "Embargo"@de ,
        "embargo"@en ;
    rdfs:comment "Verknüpft Embargo-Informationen in der KBART-Erfassungsweise."@de ,
        "Links embargo information in KBART style."@en ;
    rdfs:seeAlso "ERMI terms: _Embargo Period_ (cf. https://old.diglib.org/pubs/dlf102/ERMFINAL.pdf, p. 137)" ;
    rdfs:domain amsl:ContractItem .

amsl:erAltTitle a owl:DatatypeProperty ;
    rdfs:label "Alternativer Titel"@de ,
        "alternative title"@en ;
    rdfs:comment "Verknüpft eine Variation des Haupttitels der Ressource, z.B. Akronyme, Paralleltitel usw."@de ,
        "Links a variation of the title of the resource, including acronyms, parallel titles, titles in other languages, etc."@en ;
    rdfs:seeAlso "ERMI terms: _Electronic Resource Alternate Title_ (cf. https://old.diglib.org/pubs/dlf102/ERMFINAL.pdf, p. 134)" ;
    rdfs:domain amsl:BasicContractData .

amsl:erStatus a owl:ObjectProperty ;
    rdfs:label "Status der ER"@de ,
        "status of the ER"@en ;
    rdfs:comment "Verknüpft den Status der elektronischen Ressourcen bzw. des diese beinhaltenden Vertrages im Erwerbungsprozess"@de ,
    	"Links the status of the electronic resources resp. of the containing contract in the acquisition process."@en ;
    rdfs:seeAlso "ERMI terms: _Electronic Resource Status_ (cf. https://old.diglib.org/pubs/dlf102/ERMFINAL.pdf, p. 138)" ;
    rdfs:domain amsl:BasicContractData ;    
    rdfs:range amsl:ERStatus .

amsl:erType a owl:ObjectProperty ;
    rdfs:label "Produktart"@de ,
        "product type"@en ;
    rdfs:comment "Verknüpft die Produktart der in einem Vertrag lizenzierten elektronischen Ressourcen."@de ,
    	"Links the type of product of the electronic resources licensed in a contract."@en ;
    rdfs:seeAlso "ERMI terms: _Resource Type (cf. https://old.diglib.org/pubs/dlf102/ERMFINAL.pdf, p. 136)" ; 
    rdfs:domain amsl:BasicContractData ;
    rdfs:range amsl:ERType .

amsl:evaluateHoldingsFileFor a owl:ObjectProperty ;
    rdfs:label "Holdings-File auswerten für"@de , 
        "evaluate holdings file for"@en ;
    rdfs:comment "Verknüpft eine Einrichtung, für die ein Holdings-File ausgewertet werden soll, um die in den Katalog einzubindenden Metadatenkollektionen zu filtern."@de ,
        "Links an organizations, for which a holdings file has to be evaluated in order to filter the meta data collections, which are to be embedded in the catalogue."@en ;
    rdfs:domain amsl:MetadataCollection ;
    rdfs:range foaf:Organization .

amsl:expectedInvoiceMonth a owl:DeprecatedProperty ;
    rdfs:label "Erwarteter Rechnungsmonat"@de ,
        "expected invoice month"@en ;
    rdfs:comment "Überholt. Bitte amsl:expectedInvoiceDate nutzen."@de , 
    	"Deprecated. Please use amsl:expectedInvoiceDate."@en ;   
    rdfs:domain amsl:BasicContractData ;
    rdfs:range amsl:Month  ;
    owl:deprecated "true"^^xsd:boolean .

amsl:expectedInvoiceDate a owl:DatatypeProperty ;
    rdfs:label "Erwartetes Rechnungsdatum"@de ,
        "expected invoice date"@en ;
    rdfs:comment "Verknüpft das Datum, zu dem der Eingang der Rechnung zu einem Vertrag erwartet wird."@de , 
    	"Línks the date the invoice receipt for a contract is expected."@en ;    
    rdfs:domain amsl:AnnualContractData ;
    rdfs:range xsd:date .

amsl:expectedPrice a owl:DatatypeProperty ;
    rdfs:label "Planpreis (EUR)"@de ,
        "expected price (EUR)"@en ;
    rdfs:comment "Verknüpft den Preis, welcher für das laufende Jahr für den Vertrag geschätzt und eingeplant wurde."@de ,
        "Links the price that was expected and planned for the license for the current year."@en ;
    rdfs:domain  [ a owl:Class ;
        owl:unionOf ( amsl:AnnualContractData amsl:Subtotal ) ] ;
    rdfs:range xsd:decimal .
    
amsl:expectedPriceFollowingYear a owl:DatatypeProperty ;
    rdfs:label "Planpreis Folgejahr (EUR)"@de ,
        "expected price following year (EUR)"@en ;
    rdfs:comment "Überholt. Bitte amsl:expectedPrice mit nächstjährigen amsl:AnnualContractData nutzen."@de ,
        "Deprecated. Please use amsl:expectedPrice with next year's amsl:AnnualContractData."@en ;
    rdfs:domain amsl:AnnualContractData ;
    owl:deprecated "true"^^xsd:boolean . 

amsl:expectedPriceSubtotal a owl:ObjectProperty ;
    rdfs:label "Planpreis Teilsumme"@de ,
        "expected price subtotal"@en ;
    rdfs:comment "Verknüpft die Teilsumme eines Planpreises. Dieser wiederum kann der Betrag sowie das belastete Budget zugeordnet werden."@de ,
        "Links the subtotal of an expected price. The subtotal again may be linked with the amount due and the budget charged."@en ;
    rdfs:domain amsl:AnnualContractData ;
    rdfs:range amsl:Subtotal .

amsl:externalContact a owl:ObjectProperty ;
    rdfs:label "Externer Ansprechpartner"@de ,
        "external contact"@en ;
    rdfs:comment "Verknüpft den verantwortlichen Ansprechpartner auf Seiten von Verlagen, Konsortien, Metadatenprovidern etc."@de ,
        "Links the responsible contact person from publisher, licensing agent, consortium etc."@en ;
    rdfs:domain  [ a owl:Class ;
        owl:unionOf ( amsl:AnnualContractData amsl:MetadataSource ) ] ;
    rdfs:range foaf:Person .

amsl:faculty a owl:ObjectProperty ;
    rdfs:label "Fakultät"@de ,
        "faculty"@en ;
    rdfs:comment "Verknüpft eine bestimmte Fakultät, etwa bei Fakultätsanteilen."@de ,
        "Links a certain faculty, e.g. in the context of faculty shares."@en ;
    rdfs:range aiiso:Faculty .   

amsl:facultyAbbr a owl:DatatypeProperty ;
    rdfs:label "Fakultätskürzel"@de ,
        "faculty abbreviation"@en ;
    rdfs:comment "Verknüpft die intern gebräuchliche Abkürzung einer Fakultätsbezeichnung."@de ,
        "Links the internally common abbreviation of a faculty name."@en ;
    rdfs:domain aiiso:Faculty .   

amsl:facultyShare a owl:ObjectProperty ;
    rdfs:label "Fakultätsanteil"@de ,
        "faculty share"@en ;
    rdfs:comment "Verknüpft den Anteil an einem Vertrag, der von einer bestimmten Fakultät getragen wird."@de ,
        "Links a certain faculty's share of a license contract."@en ;
    rdfs:domain amsl:AnnualContractData ;
    rdfs:range amsl:FacultyShare .

amsl:feedbackDate a owl:DatatypeProperty ;
    rdfs:label "Rückmeldetermin"@de ,
        "feedback date"@en ;
    rdfs:comment "Verknüpft den letztmöglichen Tag, an welchem eine Rückmeldung an Zahlungsempfänger, Lizenzgeber etc. erfolgen muss."@de ,
        "Links the last possible date to give feedback to licensing agent, licensor etc."@en ;
    rdfs:seeAlso "ERMI terms: _Purchase Renewal Date_ (cf. https://old.diglib.org/pubs/dlf102/ERMFINAL.pdf, p. 142)" ;
    rdfs:domain amsl:AnnualContractData ;
    rdfs:range xsd:date .

amsl:field a owl:DatatypeProperty ;
    rdfs:label "Fachgebiet"@de ,
        "field"@en ;
    rdfs:comment "Verknüpft Fakultäten mit ihren Fachgebieten."@de ,
        "Links faculties with their field of activity."@en ;
    rdfs:domain aiiso:Faculty .

amsl:file a owl:ObjectProperty ;
    rdfs:label "Zugehörige Datei"@de ,
     "associated file"@en ;
    rdfs:comment "Verknüpft eine Ressource des Typs Dokument."@de , 
        "Links a resource of the type Document."@en   ;
    rdfs:range foaf:Document . 

amsl:fiscalYear a owl:DatatypeProperty ;
    rdfs:label "Haushaltsjahr"@de ,
        "fiscal year"@en ;
    rdfs:comment "Verknüpft das Haushaltsjahr eines Jahresbudgets."@de ,
        "Links the fiscal year of a budget."@en ;
    rdfs:domain amsl:AnnualBudget ;
    rdfs:range xsd:integer .

amsl:hasRemoteAccess a owl:ObjectProperty ;
    rdfs:label "Remote Access"@de ,
        "remote access"@en ;
    rdfs:comment "Verknüpft Informationen über das Recht eines autorisierten Nutzers, von außerhalb Zugang zu elektronischen Produkten zu erlangen."@de ,
        "Links information on the right of an authorized user to gain access to an Electronic Product from an offsite location"@en ;
    rdfs:seeAlso "ERMI terms: _Remote Access_ (cf. https://old.diglib.org/pubs/dlf102/ERMFINAL.pdf, p. 157)" ; 
    rdfs:domain amsl:BasicContractData ;
    rdfs:range amsl:ExtendedBoolean .

amsl:holdingsFile a owl:ObjectProperty ;
    rdfs:subPropertyOf amsl:file ;
    rdfs:label "Holdings-File"@de ,
        "holdings file"@en ;
    rdfs:comment "Verknüpft eine Ressource des Typs Dokument, die das aktuelle Holdings-File einer Bibliothek darstellt."@de , 
        "Links a resource of the type Document which is a library's current holdings file."@en   ;
    rdfs:seeAlso "ERMI terms: _Electronic Holdings_ (cf. https://old.diglib.org/pubs/dlf102/ERMFINAL.pdf, p. 137)" ;
    rdfs:domain foaf:Organization ;
    rdfs:range foaf:Document .     

amsl:illNote a owl:DatatypeProperty ;
    rdfs:label "Fernleihnotiz"@de ,
        "interlibrary loan note"@en ;
    rdfs:comment "Verknüpft weitere Informationen über Fernleihbedingungen."@de ,
        "Links further information on terms concerning the interlibrary loan."@en ;
    rdfs:seeAlso "ERMI terms: _Interlibrary Loan Term Note_ (cf. https://old.diglib.org/pubs/dlf102/ERMFINAL.pdf, p. 155)" ; 
    rdfs:domain amsl:BasicContractData .

amsl:illset a owl:ObjectProperty ;
    rdfs:label "Interlibrary Loan Secure Electronic Transmission"@de ,
        "interlibrary loan secure electronic transmission"@en ;
    rdfs:comment "Verknüpft Informationen über ILLSET."@de ,
    	"Links information on ILLSET."@en ; 
    rdfs:seeAlso "ERMI terms: _Interlibrary Loan Secure Electronic Transmission_ (cf. https://old.diglib.org/pubs/dlf102/ERMFINAL.pdf, p. 154)" ;       
    rdfs:domain amsl:BasicContractData ;
    rdfs:range amsl:LicenseTerm .

amsl:illElectronic a owl:ObjectProperty ;
    rdfs:label "Fernleihe elektronisch"@de ,
        "interlibrary loan electronic"@en ;
    rdfs:comment "Verknüpft Informationen über das Recht lizenziertes Material in Form einer digitalen Kopie für die Fernleihe zur Verfügung zu stellen."@de ,
        "Links information on the right to provide the licensed materials via interlibrary loan by way of electronic copies."@en ;
    rdfs:seeAlso "ERMI terms: _Interlibrary Loan Electronic_ (cf. https://old.diglib.org/pubs/dlf102/ERMFINAL.pdf, p. 155)" ; 
    rdfs:domain amsl:BasicContractData ;
    rdfs:range amsl:LicenseTerm .

amsl:illPrintOrFax a owl:ObjectProperty ;
    rdfs:label "Fernleihe print / Fax"@de ,
        "interlibrary loan print or fax"@en ;
    rdfs:comment "Verknüpft Informationen über das Recht lizenziertes Material in Form einer Print- oder Faxkopie für die Fernleihe zur Verfügung zu stellen."@de ,
        "Links information on the right to provide the licensed materials via interlibrary loan by way of print copies or facsimile transmission."@en ;
    rdfs:seeAlso "ERMI terms: _Interlibrary Loan Print or Fax_ (cf. https://old.diglib.org/pubs/dlf102/ERMFINAL.pdf, p. 154)" ; 
    rdfs:domain amsl:BasicContractData ;
    rdfs:range amsl:LicenseTerm .

amsl:includedInMetadataSource a owl:ObjectProperty ;
    rdfs:label "enthalten in Metadatenquelle"@de ,
        "included in metadata source"@en ;
    rdfs:comment "Verknüpft die die Kollektion enthaltende Metadatenquelle."@de ,
        "Links the metadata source including the collection."@en ;
    rdfs:domain amsl:MetadataCollection ;
    rdfs:range amsl:MetadataSource .

amsl:indexingLevel a owl:DatatypeProperty ;
    rdfs:label "Indexierungsgrad"@de ,
        "indexing level"@en ;
    rdfs:comment "Verknüpft Angaben zum gebotenen Indexierungsgrad"@de ,
        "Links information on the indexing level offered."@en ;
    rdfs:domain amsl:MetadataSource .

amsl:individualContractItems a owl:ObjectProperty ;
    rdfs:label "Individuelle Vertragspositionen"@de ,
        "individual contract items"@en ;
    rdfs:comment "Gibt an, ob ein konsortialer Vertrag unterschiedliche Vertragspositionen für verschiedene teilnehmende Bibliotheken umfassen kann. Falls dies der Fall ist, müssen Pakete und Vertragspositionen jeweils in der lokelen Wissensbasis jeder Bibliothek erfasst werden."@de ,
        "Indicates if a consortial contract can have individual contract items for different participating libraries. If this is the case, license packages and contract items need to be recorded in the local ERM knowledge base of each library."@en ;
    rdfs:domain amsl:BasicContractData ;
    rdfs:range amsl:Boolean .

amsl:initialAcquisitionDate a owl:DatatypeProperty ;
    rdfs:label "Ersterwerbungsdatum"@de ,
        "initial acquisition date"@en ;
    rdfs:comment "Verknüpft das Datum, an welchem das Produkt zum ersten Mal erworben wurde."@de ,
        "Links the date the license was purchased by the licensee for the first time."@en ;
    rdfs:domain amsl:BasicContractData ;
    rdfs:range xsd:date .

amsl:internalContact a owl:ObjectProperty ;
    rdfs:label "Hausinterner Ansprechpartner"@de ,
        "inhouse contact"@en ;
    rdfs:comment "Verknüpft den verantwortlichen Ansprechpartner auf Seiten des Lizenznehmers."@de ,
        "Links the responsible inhouse contact person for the contract."@en ;
    rdfs:domain  [ a owl:Class ;
        owl:unionOf ( amsl:BasicContractData amsl:MetadataSource ) ] ;
    rdfs:range foaf:Person .

amsl:invoiceProcessingDate a owl:DatatypeProperty ;
    rdfs:label "Rechnungsbearbeitungsdatum"@de ,
        "invoice processing date"@en ;
    rdfs:comment "Verknüpft den Tag, an dem die Rechnung bearbeitet wurde."@de ,
        "Links the day the invoice was processed."@en ;
    rdfs:domain amsl:AnnualContractData ;
    rdfs:range xsd:date .

amsl:invoiceDate a owl:DatatypeProperty ;
    rdfs:label "Rechnungsdatum"@de ,
        "invoice date"@en ;
    rdfs:comment "Verknüpft das Datum, an dem die Rechnung erstellt wurde."@de ,
        "Links the day the invoice was created."@en ;
    rdfs:domain amsl:AnnualContractData ;
    rdfs:range xsd:date .
  
amsl:invoiceFile a owl:ObjectProperty ;
    rdfs:subPropertyOf amsl:file ;
    rdfs:label "Rechnungsdatei"@de ,
        "invoice file"@en ;
    rdfs:comment "Verknüpft eine Ressource des Typs Dokument."@de , 
        "Links a resource of the type Document."@en   ;
    rdfs:domain amsl:AnnualContractData ;
    rdfs:range foaf:Document .

amsl:invoicePriceGrossEUR  a owl:DatatypeProperty ;
	rdfs:label "Rechnungspreis brutto (EUR)"@de ,
		"invoice price gross (EUR)"@en ;
	rdfs:comment "Verknüpft den brutto Rechnungspreis in Euro."@de ,
		"Links the invoice price gross in euro."@en ;
	rdfs:domain  [ a owl:Class ;
        owl:unionOf ( amsl:AnnualContractData amsl:Subtotal ) ] ;
    rdfs:range xsd:decimal .

amsl:invoicePriceGrossGBP a owl:DatatypeProperty;
    rdfs:label "Rechnungspreis brutto (GBP)"@de ,
        "invoice price gross (GBP)"@en ;
    rdfs:comment "Verknüpft den brutto Rechnungspreis in Pfund Sterling."@de ,
        "Links the invoice price gross in pound sterling."@en ;
    rdfs:domain  [ a owl:Class ;
        owl:unionOf ( amsl:AnnualContractData amsl:Subtotal ) ] ;
    rdfs:range xsd:decimal .

amsl:invoicePriceGrossUSD a owl:DatatypeProperty;
	rdfs:label "Rechnungspreis brutto (USD)"@de ,
		"invoice price gross (USD)"@en ;
	rdfs:comment "Verknüpft den brutto Rechnungspreis in US-Dollar."@de ,
		"Links the invoice price gross in US-Dollar."@en ;
    rdfs:domain  [ a owl:Class ;
        owl:unionOf ( amsl:AnnualContractData amsl:Subtotal ) ] ;
    rdfs:range xsd:decimal .

amsl:invoicePriceNetEUR a owl:DatatypeProperty;
    rdfs:label "Rechnungspreis netto (EUR)"@de ,
        "invoice price net (EUR)"@en ;
    rdfs:comment "Verknüpft den netto Rechnungspreis in Euro."@de ,
        "Links the invoice price net in euro."@en ;
    rdfs:domain  [ a owl:Class ;
        owl:unionOf ( amsl:AnnualContractData amsl:Subtotal ) ] ;
    rdfs:range xsd:decimal .

amsl:invoicePriceNetGBP  a owl:DatatypeProperty;
    rdfs:label "Rechnungspreis netto (GBP)"@de ,
        "invoice price net (GBP)"@en ;
    rdfs:comment "Verknüpft den netto Rechnungspreis in Pfund Sterling."@de ,
        "Links the invoice price net in pound sterling."@en ;
    rdfs:domain  [ a owl:Class ;
        owl:unionOf ( amsl:AnnualContractData amsl:Subtotal ) ] ;
    rdfs:range xsd:decimal .

amsl:invoicePriceNetUSD a owl:DatatypeProperty;
    rdfs:label "Rechnungspreis netto (USD)"@de ,
        "invoice price net (USD)"@en ;
    rdfs:comment "Verknüpft den netto Rechnungspreis in US-Dollar."@de ,
        "Links the invoice price net in US-Dollar."@en ;
    rdfs:domain  [ a owl:Class ;
        owl:unionOf ( amsl:AnnualContractData amsl:Subtotal ) ] ;
    rdfs:range xsd:decimal .      

amsl:invoicePriceSubtotal a owl:ObjectProperty ;
    rdfs:label "Rechnungspreis Teilsumme"@de ,
        "invoice price subtotal"@en ;
    rdfs:comment "Verknüpft die Teilsumme eines Rechnungspreises. Dieser wiederum kann der Betrag sowie das belastete Budget zugeordnet werden."@de ,
        "Links the subtotal of an invoice price. The subtotal again may be linked with the amount due and the budget charged."@en ;
    rdfs:domain amsl:AnnualContractData ;
    rdfs:range amsl:Subtotal .

amsl:invoiceReceived a owl:ObjectProperty ;
    rdfs:label "Rechnung vorhanden"@de ,
        "invoice received"@en ;
    rdfs:comment "Verknüpft die Information, ob die aktuelle Rechnung bereits eingegangen ist."@de ,
        "Links the information, if the current invoice has alreday been received."@en ;
    rdfs:domain amsl:AnnualContractData ;
    rdfs:range amsl:Boolean .
    
amsl:isMemberOf a owl:ObjectProperty ;
    rdfs:label "Mitglied von"@de ,
        "member of"@en ;
    rdfs:comment "Verknüpft die Organisation, bei der eine Person Mitglied ist."@de ,
    	"Links the organization a person is a member of."@en ;
    rdfs:seeAlso "ERMI terms: _Organization Represented_ (cf. https://old.diglib.org/pubs/dlf102/ERMFINAL.pdf, p. 205)" ;
    rdfs:domain [ a owl:Class ;
        owl:unionOf ( foaf:Person sioc:User ) ] ;
    rdfs:range foaf:Organization . 

amsl:isRelatedTo a owl:ObjectProperty ;
    rdfs:label "thematisch zugehörig zu"@de ,
    	"related to"@en ;
    rdfs:comment "Verknüpft eine elektronische Ressourcen über deren ISSN mit einer thematisch passend zum Inhalt der Ressource ausgerichteten Fakultät."@de ,
    	"Links an electronic resource via its ISSN with an thematically related faculty."@en ;    	
    rdfs:range aiiso:Faculty .

amsl:itemPrice a owl:DatatypeProperty ;
    rdfs:label "Preis einzelner Titel (EUR)"@de ,
        "price single title (EUR)"@en ;
    rdfs:comment "Verknüpft den Anschaffungs-/Nutzungspreis, den die Bibliothek für eine Bibliographische Ressource bezahlt."@de ,
        "Links the acquisition/usage price for a bibliographic resource."@en ;
    rdfs:domain amsl:ContractItem ;
    rdfs:range xsd:decimal .

amsl:licensee a owl:ObjectProperty ;
    rdfs:label "Lizenznehmer"@de ,
        "licensee"@en ;
    rdfs:comment "Verknüpft die Vertragspartei, die eine Lizenz erhält."@de ,
        "Links the contracting party obtaining the license."@en ;
    rdfs:seeAlso "ERMI terms: _Licensee_ (cf. https://old.diglib.org/pubs/dlf102/ERMFINAL.pdf, p. 148)" ; 
    rdfs:domain amsl:BasicContractData ;
    rdfs:range foaf:Organization .    

amsl:licenseEndDate a owl:DatatypeProperty ;
    rdfs:label "Vertragsende"@de ,
        "license end date"@en ;
    rdfs:comment "Verknüpft das Datum, an welchem die Gültigkeit eines Lizenzvertrags endet"@de ,
        "Links the date on which a license agreement terminates"@en ;
    rdfs:seeAlso "ERMI terms: _License End Date_ (cf. https://old.diglib.org/pubs/dlf102/ERMFINAL.pdf, p. 147)" ; 
    rdfs:domain amsl:AnnualContractData ;
    rdfs:range xsd:date .

amsl:licenseStartDate a owl:DatatypeProperty ;
    rdfs:label "Vertragsbeginn"@de ,
        "license start date"@en ;
    rdfs:comment "Verknüpft das Datum, an welchem ein Lizenzvertrag in Kraft tritt."@de ,
        "Links the date on which a license agreement comes into effect."@en ;
    rdfs:seeAlso "ERMI terms: _License Start Date_ (cf. https://old.diglib.org/pubs/dlf102/ERMFINAL.pdf, p. 147)" ; 
    rdfs:domain amsl:AnnualContractData ;
    rdfs:range xsd:date .

amsl:licenseType a owl:ObjectProperty,
        owl:ObjectProperty ;
    rdfs:label "Lizenzart"@de ,
        "license type"@en ;
    rdfs:comment "Verknüpft Informationen über die Art der Lizenz, welche den Zugang zu der elektronischen Ressource regelt."@de ,
        "Links information on the type of license that regulates access to the electronic resource."@en ;
    rdfs:domain amsl:AnnualContractData ;
    rdfs:range amsl:LicenseType .

amsl:licensingAgent a owl:ObjectProperty ;
    rdfs:label "Zahlungsempfänger"@de ,
        "licensing agent"@en ;
    rdfs:comment "Verknüpft ein Unternehmen, das die Bezahlung einer ER abwickelt."@de ,
    "Links an organization (such as a subscription agent) that facilitates a licensing transaction on behalf of one or more parties."@en ;
    rdfs:seeAlso "ERMI terms: _Licensing Agent_ (cf. https://old.diglib.org/pubs/dlf102/ERMFINAL.pdf, p. 148)" ; 
    rdfs:domain amsl:AnnualContractData ;
    rdfs:range foaf:Organization .

amsl:licensingNote a owl:DatatypeProperty ;
    rdfs:label "Bemerkungen zum Vertrag"@de ,
        "licensing note"@en ;
    rdfs:comment "Verknüpft zusätzliche Informationen, welche den Vertrag, die Lizenzverhandlungen, das Produkt etc. betreffen."@de ,
        "Links additional information regarding the license, the negotiation of the license, the product, etc."@en ;
    rdfs:seeAlso "ERMI terms: _Licensing Note_ (cf. https://old.diglib.org/pubs/dlf102/ERMFINAL.pdf, p. 146)" ; 
    rdfs:domain [ a owl:Class ;
        owl:unionOf ( amsl:AnnualContractData amsl:MetadataSource ) ] .

amsl:licensor a owl:ObjectProperty ;
    rdfs:label "Lizenzgeber"@de ,
        "licensor"@en ;
    rdfs:comment "Verknüpft die Vertragspartei, die eine Lizenz zur Verfügung stellt."@de ,
        "Links the contracting party granting the license."@en ;
    rdfs:seeAlso "ERMI terms: _Licensor_ (cf. https://old.diglib.org/pubs/dlf102/ERMFINAL.pdf, p. 148)" ; 
    rdfs:domain amsl:BasicContractData ;
    rdfs:range foaf:Organization .

amsl:linkToBalance a owl:DatatypeProperty ;
    rdfs:label "Link zum Über-/Fehlbetrag"@de ,
        "link to balance"@en ;
    rdfs:comment "Verknüpft einen Link zum Über-/Fehlbetrag."@de ,
        "Links a hyperlink to the balance."@en ;    
    rdfs:domain amsl:AnnualContractData .

amsl:linkToContentFile a owl:DatatypeProperty ;
    rdfs:label "Link zum Content-File"@de ,
        "link to content file"@en ;
    rdfs:comment "Verknüpft den Downloadlink eines Content-Files."@de ,
        "Links the download link to a content file."@en ;
    rdfs:domain [ a owl:Class ;
        owl:unionOf ( amsl:MetadataCollection amsl:LicensePackage ) ] .   

amsl:linkToContract a owl:DatatypeProperty ;
    rdfs:label "Link zum Vertrag"@de ,
        "link to contract"@en ;
    rdfs:comment "Verknüpft einen Link/eine URL, die auf die digitale Version das originalen Vertragsdokuments verweist, welches der Lizenznehmer vom Lizenzgeber enthält."@de ,
        "Links a url linking to a digital version of the original contract document the licensee received from the licensor."@en ;
    rdfs:seeAlso "ERMI terms: _License Uniform Resource Identifier_ (cf. https://old.diglib.org/pubs/dlf102/ERMFINAL.pdf, p. 145)" ;  
    rdfs:domain amsl:AnnualContractData .

amsl:linkToDescription a owl:DatatypeProperty ;
    rdfs:label "URL der Anbieterbeschreibung"@de ,
        "link to description "@en ;
    rdfs:comment "Verknüpft einen Link zur Beschreibung der ER des Anbieter.s"@de ,
        "Links the URL to the description of the creator/provider of an Electronic Product."@en ;
    rdfs:domain amsl:BasicContractData .

amsl:linkToHoldingsFile a owl:DatatypeProperty ;
    rdfs:label "Link zum Holdings-File"@de ,
        "link to holdings file"@en ;
    rdfs:comment "Verknüpft den Downloadlink zu dem aktuellen Holdings-File einer Bibliothek."@de ,
        "Links the Download link to a library's current holdings file."@en ;
    rdfs:domain foaf:Organization .    

amsl:linkToInvoice a owl:DatatypeProperty ;
    rdfs:label "Link zur Rechnung"@de ,
        "link to invoice"@en ;
    rdfs:comment "Verknüpft einen Link zur Rechnung."@de ,
        "Links a hyperlink to the invoice."@en ;    
    rdfs:domain amsl:AnnualContractData .

amsl:localSystemNumber a owl:DatatypeProperty ;
    rdfs:label "Nummer aus Lokalsystem"@de ,
        "local system number"@en ;
    rdfs:comment "Verknüpft eine Nummer, die das lokale Bibliotheksmanagementsystem (z.B. Libero) für die Ressource vergibt."@de ,
        "Links the record number that is assigned by a local integrated library system (ILS) to the bibliographic record for the resource."@en ;
    rdfs:seeAlso "ERMI terms: _Local System Number_ (cf. https://old.diglib.org/pubs/dlf102/ERMFINAL.pdf, p. 133)" ;
    rdfs:domain [ a owl:Class ;
    	owl:unionOf ( amsl:AnnualContractData amsl:ContractItem  amsl:LicensePackage ) ] .

amsl:mailFile a owl:ObjectProperty ;
    rdfs:subPropertyOf amsl:file ;
    rdfs:label "Schriftverkehrsdatei"@de ,
        "mail file"@en ;
    rdfs:comment "Verknüpft eine Ressource des Typs Dokument, die eine Schriftverkehrsdatei ."@de , 
        "Links a resource of the type Document."@en   ;
    rdfs:domain [ a owl:Class ;
        owl:unionOf ( amsl:BasicContractData amsl:AnnualContractData ) ] ;
    rdfs:range foaf:Document .        

amsl:metadataSourceImplStatus a owl:ObjectProperty ;
    rdfs:label "Status der Metadaten-Implementierung"@de ,
        "metatadata implementation status"@en ;
    rdfs:comment "Verknüpft Informationen über den Status der Implementierung der Metadatenquelle im Artikelindex."@de ,
        "Links information on the implementation status of the metadata source in the article index."@en ;
    rdfs:domain amsl:MetadataSource ;
    rdfs:range amsl:MetadataSourceImplStatus .

amsl:metadataUsedByLibrary a owl:ObjectProperty;
    rdfs:label "Metadaten nutzende Bibliothek"@de ,
        "metadata used by library"@en ;
    rdfs:comment "Verknüpft die Bibliothek, die die Metadaten einer Kollektion nutzt."@de ,
        "Links the library using a collection's metadata."@en ;
    rdfs:domain amsl:MetadataCollection ;
    rdfs:range foaf:Organization .

amsl:metadataUsagePermittedForLibrary a owl:ObjectProperty ;
    rdfs:label "Metadatennutzung erlaubt für"@de ,
         "metadata usage permitted for" ;
    rdfs:comment "Verknüpft eine Bibliothek, der die Nutzung einer an Metadatenkollektion mit eingeschränkter Nutzung erlaubt ist."@de , 
        "Links a library that has the permission to use a usage-restricted metadata collection."@en ;
    rdfs:domain amsl:MetadataCollection ;
    rdfs:range foaf:Organization .

amsl:metadataUsageProhibited a owl:ObjectProperty ;
    rdfs:label "Metadatennutzung untersagt"@de ,
         "metadata usage prohibited" ;
    rdfs:comment "Verknüpft eine Bibliothek, der die Nutzung einer bestimmten Metadatenkollektion z. B. aus lizenzrechtlichen Gründen untersagt ist."@de , 
        "Links a library that is prohibited from using a certain metadata collection due to e.g. licensing restrictions."@en ;
    rdfs:domain amsl:MetadataCollection ;
    rdfs:range foaf:Organization ;
    owl:deprecated "true"^^xsd:boolean .

amsl:metadataUsageRestricted a owl:ObjectProperty ;
    rdfs:label "Metadatennutzung eingeschränkt"@de ,
         "metadata usage restricted" ;
    rdfs:comment "Gibt an, ob die Nutzung einer bestimmten Metadatenkollektion z. B. aus lizenzrechtlichen Gründen eingeschränkt ist."@de , 
        "States if a certain metadata collection has restricted usage due to e.g. licensing reasons."@en ;
    rdfs:domain amsl:MetadataCollection ;
    rdfs:range amsl:Boolean .

amsl:nextUpdateDate a owl:DatatypeProperty ;
    rdfs:label  "Datum des nächsten Updates"@de ,
        "date of next update"@en ;
    rdfs:comment "Verknüpft das Datum der nächsten Aktualisierung der angebotenen Metadaten"@de , 
        "Links the date of the next update of the offered metadata."@en ;
    rdfs:domain amsl:Source ;
    rdfs:range xsd:date .    

amsl:noticePeriod a owl:DatatypeProperty ;
    rdfs:label "Kündigungsfrist"@de ,
        "notice period"@en ;
    rdfs:comment "Verknüpft die einzuhaltende Kündigungsfrist eines Vertrages. Die Kündigungsfrist ist zu verwenden, wenn die vorliegenden Angaben kein Datum darstellen oder nicht sinnvoll in ein solches umgerechnet werden können."@de ,
        "Links the the notice period to be adhered. The notice period must be recorded if no exact date can be identified."@en ;
    rdfs:domain amsl:AnnualContractData .

amsl:numberFirstIssueOnline a owl:DatatypeProperty ;
   rdfs:label "Nummer erster online verfügbarer Ausgabe"@de ,
        "number of first issue available online"@en ;
    skos:prefLabel  "Nr. erste verf. Ausg."@de ,
        "no. first issue avail."@en ;
    rdfs:comment "Verknüpft die Nummer der ersten online verfügbaren Ausgabe eines E-Journals. Angabe ohne Bandbezeichnungen (z.B. 'Nr.' oder 'Heft')."@de ,
        "Links the number of the first issue of an e-journal available online. Do not include any labels (e.g., 'no.' or 'n.') nor any supplement or part values."@en ;
    rdfs:domain amsl:ContractItem  . 

amsl:numberFirstVolumeOnline a owl:DatatypeProperty ;
    rdfs:label "Nummer des ersten online verfügbaren Jahrganges"@de ,
        "number of first volume available online"@en ;
    skos:prefLabel  "Nr. erster verf. Jg."@de ,
        "no. first vol. avail."@en ;
    rdfs:comment "Verknüpft die Nummer des ersten online verfügbaren Jahrganges eines E-Journals. Angabe ohne Bandbezeichnungen (z.B. 'Bd.' oder 'Jg.')."@de ,
        "Links the number of the first volume of an e-journal available online. Do not include any labels (e.g., 'vol.' or 'v.')."@en ;
    rdfs:domain amsl:ContractItem  . 

amsl:numberLastIssueOnline a owl:DatatypeProperty ;
    rdfs:label "Nummer letzter online verfügbarer Ausgabe"@de ,
        "number of last issue available online"@en ;
    skos:prefLabel  "Nr. letzte verf. Ausg."@de ,
        "no. last issue avail."@en ;
    rdfs:comment "Verknüpft die Nummer der letzten online verfügbaren Ausgabe eines E-Journals. Angabe ohne Bandbezeichnungen (z.B. 'Nr.' oder 'Heft')."@de ,
        "Links the number of the last issue of an e-journal available online. Do not include any labels (e.g., 'no.' or 'n.') nor any supplement or part values."@en ;
    rdfs:domain amsl:ContractItem  . 

amsl:numberLastVolumeOnline a owl:DatatypeProperty ;
    rdfs:label "Nummer letzten online verfügbaren Jahrganges"@de ,
        "number of last volume available online"@en ;
    skos:prefLabel  "Nr. letzter verf. Jg."@de ,
        "no. last vol. avail."@en ;
    rdfs:comment "Verknüpft die Nummer des letzten online verfügbaren Jahrganges eines E-Journals. Angabe ohne Bandbezeichnungen (z.B. 'Bd.' oder 'Jg.')."@de ,
        "Links the number of the last volume of an e-journal available online. Do not include any labels (e.g., 'vol.' or 'v.')."@en ;
    rdfs:domain amsl:ContractItem  . 

amsl:organizationType a owl:ObjectProperty ;
    rdfs:label "Kategorie"@de ,
        "organization type"@en ;
    rdfs:comment "Verknüpft die Kategorie einer Organisation."@de ,
        "Links the category resp. type of an organization."@en ;    
    rdfs:domain foaf:Organization ;
    rdfs:range amsl:OrganizationType .

amsl:orgNote a  owl:DatatypeProperty ;
    rdfs:label "Notiz zur Organisation"@de ,
        "organization note"@en ;
    rdfs:comment "Verknüpft weitere Informationen zu einer Organisation."@de ,
    	"Links further information on an organization."@en ; 
    rdfs:seeAlso "ERMI terms: _Organization Note_ (cf. https://old.diglib.org/pubs/dlf102/ERMFINAL.pdf, p. 204)" ; 
    rdfs:domain foaf:Organization .

amsl:paymentPeriod  a owl:ObjectProperty ;
    rdfs:label "Zahlungszeitraum"@de ,
        "payment period"@en ;
    rdfs:comment "Verknüpft den Zeitraum, in dem die Zahlung einer Rechnung fällig wird."@de ,
        "Línks the period the payment of an invoice is due."@en ;
    rdfs:domain amsl:AnnualContractData ;
    rdfs:range amsl:PaymentPeriod .       

amsl:pCopy a owl:ObjectProperty ;
    rdfs:label "Kopie print"@de ,
        "print copy "@en ;
    rdfs:comment "Verknüpft Informationen üas Recht des Lizenznehmers und autorisierter Nutzer, eine gedruckte Kopie zu erstellen."@de ,
        "links information on the right of the licensee and authorized users to make a printed copy of the licensed resource."@en ;
    rdfs:seeAlso "ERMI terms: _Print Copy_ (cf. https://old.diglib.org/pubs/dlf102/ERMFINAL.pdf, p. 153)" ; 
    rdfs:domain amsl:BasicContractData ;
    rdfs:range amsl:LicenseTerm .

amsl:percentage a owl:DatatypeProperty ;
    rdfs:label "prozentualer Anteil"@de ,
        "percentage"@en ;
    rdfs:comment "Verknüpft einen prozetualen Anteil, etwa bei Fakultätsanteilen."@de ,
        "Links a percentage, e.g. in the context of faculty shares."@en ;
    rdfs:range xsd:decimal .

amsl:pisbn a owl:ObjectProperty ;
    rdfs:label "P-ISBN"@de ,
        "P-ISBN"@en ;
    rdfs:comment "Verknüpft die P-ISBN eines Mediums."@de ,
        "Links the P-ISBN of a medium."@en ;
    rdfs:seeAlso "ERMI terms: Print International Standard Book Number_ (cf. https://old.diglib.org/pubs/dlf102/ERMFINAL.pdf, p. 209)" .  
        
amsl:pissn a owl:ObjectProperty ;
    rdfs:label "P-ISSN"@de ,
        "P-ISSN"@en ;
    rdfs:comment "Verknüpft die P-ISSN eines Mediums."@de ,
        "Links the P-ISSN of a medium."@en ;
    rdfs:seeAlso "ERMI terms: _Print International Standard Serial Number_ (cf. https://old.diglib.org/pubs/dlf102/ERMFINAL.pdf, p. 209)" .         

amsl:platform a  owl:ObjectProperty ;
    rdfs:label "Plattform"@de ,
        "platform"@en ;
    rdfs:comment "Verknüpft die Vertragsbasisdaten mit der Plattform, über die die Inhalte abrufbar sind."@de ,
        "Links basic contract data with the associated platform."@en ;
    rdfs:domain amsl:BasicContractData ;
    rdfs:range amsl:Platform .
    
amsl:previousContract a owl:ObjectProperty ;
    rdfs:label "Vorgängervertrag"@de ,
    	"previous contract"@en ;
    rdfs:comment "Verknüpft vorhergehende Vertragsbasisdaten, die mit den jetzigen in Beziehung stehen."@de ,
    	"Links previous basic cobtract data that are related to the current."@en ;
    rdfs:seeAlso "ERMI terms: _License Replaces_ (cf. https://old.diglib.org/pubs/dlf102/ERMFINAL.pdf, p. 149)" ; 
    rdfs:domain amsl:BasicContractData ;
    rdfs:range amsl:BasicContractData .    

amsl:primaryAccessURI a  owl:DatatypeProperty ;
    rdfs:label "Zugangs-URL"@de ,
        "access URL"@en ;
    rdfs:comment "Verknüpft die URI, unter der die lizenzierten Pridukte primär zugänglich sind."@de ,
        "Links the URI under which the licensed products are primarily accessible."@en ;
    rdfs:seeAlso "ERMI terms: _Primary Access Uniform Resource Identifier_ (cf. https://old.diglib.org/pubs/dlf102/ERMFINAL.pdf, p. 182)" ; 
    rdfs:domain [ a owl:Class ;
        owl:unionOf ( amsl:BasicContractData amsl:MetadataSource ) ] .

amsl:productISIL a owl:DatatypeProperty ;
    rdfs:label "Produkt-ISIL"@de ,
        "product ISIL"@en ;
    rdfs:comment "Verknüpft einen Produkt-ISIL für Pakete elektronischer Ressourcen mit deutschlandweitem Zuschnitt."@de ,
        "Links a product ISIL for packages of electronic resources laid out for German organizations"@en ;
    rdfs:domain [ a owl:Class ;
        owl:unionOf ( amsl:MetadataCollection amsl:LicensePackage ) ]  .    

amsl:proprietaryID a owl:DatatypeProperty ;
    rdfs:label "Proprietäre ID"@de ,
        "proprietary ID"@en ;
    rdfs:comment "Verknüpft einen proprietären Identifier eines Mediums."@de ,
        "Links a proprietary identifier of a medium."@en .

amsl:relatedContract a owl:ObjectProperty ;
    rdfs:label "In Beziehung stehender Vertrag"@de ,
        "related contract"@en ;
    rdfs:comment "Verknüpft einen in Beziehung stehenden Vertrag, beispielsweise ein Vertrag einer anderen Organisation."@de ,
        "Links a related contract, for example a contract of another organisation."@en ;
    rdfs:domain amsl:ContractData ;
    rdfs:range amsl:ContractData .
 
amsl:scholarlySharing a owl:ObjectProperty ;
    rdfs:label "Scholarly Sharing "@de ,
        "scholarly sharing "@en ;
    rdfs:comment "Verknüpft Informationen über das Recht des Lizenznehmers und autorisierter Nutzer, eine gedruckte oder digitale Kopie für Dritte zum persönlichen, wissenschaftlichen, bildendem oder beruflichen Gebrauch zu erstellen."@de ,
        "Links information on the right of authorized users and/or the licensee to transmit hard copy or an electronic copy of a portion of the licensed materials to a third party for personal, scholarly, educational, scientific or professional use."@en ;
    rdfs:seeAlso "ERMI terms: _Scholarly Sharing_ (cf. https://old.diglib.org/pubs/dlf102/ERMFINAL.pdf, p. 153)" ;         
    rdfs:domain amsl:BasicContractData ;
    rdfs:range amsl:LicenseTerm .

amsl:shibbolethImplStatus a owl:ObjectProperty ;
    rdfs:label "Status Shibboleth Implementation"@de ,
        "shibboleth implementation status"@en ;
    rdfs:comment "Verknüpft Informationen über den Status der Shibboleth Implementation."@de ,
        "Links information on the status of the shibboleth implementation."@en ;
    rdfs:domain amsl:Platform ;
    rdfs:range amsl:ShibbolethImplStatus .

amsl:shutDownDate a owl:DatatypeProperty ;
    rdfs:label "Abschalttermin"@de ,
        "shutdown date"@en ;
    rdfs:comment "Verknüpft das Datum, an dem der technische Zugang zum elektronischen Produkt endet."@de ,
        "Links the date the access to the ER shuts down."@en ;
    rdfs:domain amsl:BasicContractData ;
    rdfs:range xsd:date .

amsl:solrShard a owl:ObjectProperty ;
    rdfs:label "Solr-Shard"@de ,
        "solr shard"@en ;
    rdfs:comment "Verknüpft den Solr-Shard einer Metadatenquelle."@de ,
        "Links the solr shard of a metadata source."@en ;
    rdfs:domain amsl:MetadataSource ;
    rdfs:range amsl:SolrShard .

amsl:sourceID a owl:DatatypeProperty ;
    rdfs:label "Source ID"@de ,
        "source ID"@en ;
    rdfs:comment "Verknüpft die Source ID einer Metadatenquelle."@de , 
        "Links the source ID of a metadata source."@en ;
    rdfs:domain amsl:Source ;
    rdfs:range xsd:integer .

amsl:terminationAlert a owl:DatatypeProperty ;
    rdfs:label "Letztmöglicher Kündigungstag"@de ,
        "last possible termination date"@en ;
    rdfs:comment "Verknüpft das letztmögliche Datum, an welchem ein Vertrag/Abo gekündigt werden kann"@de ,
        "Links the last possible date on which a contract/subscription can be terminated"@en ;
    rdfs:domain amsl:AnnualContractData ;
    rdfs:range xsd:date .

amsl:terminationDate a owl:DatatypeProperty ;
    rdfs:label "Kündigungsdatum"@de ,
        "termination date"@en ;
    rdfs:comment "Verknüpft das Datum, an welchem ein Vertrag/Abo gekündigt worden ist."@de ,
        "Links the date a contract/subscription has been terminated."@en ;
    rdfs:seeAlso "ERMI terms: _Termination Date_ (cf. https://old.diglib.org/pubs/dlf102/ERMFINAL.pdf, p. 143)" ;
    rdfs:domain amsl:BasicContractData ;
    rdfs:range xsd:date .

amsl:terminationReason a owl:DatatypeProperty ;
    rdfs:label "Kündigungsgrund"@de ,
        "termination reason"@en ;
    rdfs:comment "Verknüpft den Grund für die Kündigung eines Vertrags."@de ,
        "Links the reason a subscription was terminated."@en ;
    rdfs:seeAlso "ERMI terms: _Termination Reason_ (cf. https://old.diglib.org/pubs/dlf102/ERMFINAL.pdf, p. 143)" ;
    rdfs:domain amsl:BasicContractData .

amsl:ticketURL a owl:ObjectProperty ;
    rdfs:label "Ticket-URL"@de ,
        "ticket URL"@en ;
    rdfs:comment "Verknüpft die URL des korrespondierenden Tickets in einem internen Ticketsystem."@de ,
        "Links the URL of a corresponding ticket in an internal ticket system."@en ;
    rdfs:domain  [ a owl:Class ;
        owl:unionOf ( amsl:MetadataSource amsl:MetadataCollection ) ] .

amsl:updateRhythm a owl:DatatypeProperty ;
    rdfs:label  "Update-Rhythmus"@de ,
        "update rhythm"@en ;
    rdfs:comment "Verknüpft Angaben zum Aktualiserungsrhythmus der angebotenen Metadaten."@de , 
        "Links information on the update rhythm of the offered metadata."@en ;
    rdfs:seeAlso "ERMI terms: _Update Frequency_ (cf. https://old.diglib.org/pubs/dlf102/ERMFINAL.pdf, p. 136)" ;
    rdfs:domain amsl:Source .    

amsl:usageStatsNote a owl:DatatypeProperty ;
    rdfs:label "Nutzungsstatistik Notiz"@de ,
        "usage statistics note"@en ;
    rdfs:comment "Verknüpft allgemeine Informationen zu Nutzungsstatistiken. Empfehlung: Angabe von Jahr, Reportform, Nutzungszahl und Link zur entsprechenden Tabelle."@de ,
        "Links general information regarding usage statistics."@en ;
    rdfs:seeAlso "ERMI terms: _Usage Statistics Note_ (cf. https://old.diglib.org/pubs/dlf102/ERMFINAL.pdf, p. 192)" ; 
    rdfs:domain amsl:AnnualContractData .

amsl:workflowStatus a owl:ObjectProperty ;
    rdfs:label "Status im Geschäftsgang"@de ,
        "workflow status"@en ;
    rdfs:comment "Verknüpft Informationen zu dem Status des Jahresvertrages im Geschäftsgang, ob ein Vertrag etwa bereits verlängert wurde oder ob die Verhandlungen dazu noch laufen."@de ,
        "Links information on the workflow status of an annual contract, e. g. that a contract has already been renewed or that the negotiations are still ongoing."@en ;
    rdfs:seeAlso "ERMI terms: _Renewal Status_ (cf. https://old.diglib.org/pubs/dlf102/ERMFINAL.pdf, p. 143)" ;
    rdfs:domain amsl:AnnualContractData ;
    rdfs:range amsl:WorkflowStatus . 


###  NEW: integration of EZB holdings import ###

amsl:HoldingsItem a owl:Class;
    rdfs:label "Bestandsposition"@de , 
       "Holdings item"@en ;
    rdfs:comment "Ein Teil des Bibliotheksbestandes, d.h. ein Medium, welches eine Bibliothek besitzt oder an welchem sie Nutzungsrechte innehat."@de ,
        "An item of the library holdings, i.e. a medium which a library owns or holds usagage rights on."@en .

amsl:ezbAnchor a owl:DatatypeProperty ;
    rdfs:label "EZB-Anker"@de , 
        "EZB anchor"@en ;
    rdfs:comment "Verknüpft ein Paket mit dessen in der EZB vergebenem Anker."@de ,
        "Links a license package with the corresponding ezb achor."@en ;
    rdf:rdfs:domain amsl:LicensePackage .

amsl:holdingsItemOf a owl:ObjectProperty ;
    rdfs:label "Bestandsposition von"@de ,
        "holdings item of"@en ;
    rdfs:comment "Verknüpft eine bestimmte Bestandsposition mit dem Lizenzpaket, in dem sie enthalten ist."@de ,
        "Links a certain holdings item with the license package it is contained in."@en ;
    rdf:rdfs:domain amsl:HoldingsItem .

amsl:ezbTitleID a owl:DatatypeProperty ;
    rdfs:label "EZB-Titel-ID"@de , 
        "EZB title id"@en ;
    rdfs:comment "Verknüpft eine Bestandsposition mit ihrer in der EZB vergebenen Titel-ID."@de ,
        "Links a holdings item with the corresponding EZB title id."@en ;
    rdf:rdfs:domain amsl:HoldingsItem .

amsl:zdbID a owl:DatatypeProperty ;
    rdfs:label "ZDB-ID"@de , 
        "ZDB id"@en ;
    rdfs:comment "Verknüpft eine Bestandsposition mit ihrer in der ZDB vergebenen ID."@de ,
        "Links a holdings item with the corresponding ZDB id."@en ;
    rdf:rdfs:domain amsl:HoldingsItem .

   
######################## Collections & Individuals #####################################
    
amsl:AcqNote a owl:Class ;
    owl:oneOf ( amsl:AllianceLicense amsl:OACharges amsl:DedicatedLicense amsl:Gift amsl:Purchase amsl:ConsortialLicense amsl:NationalLicense amsl:ScientificInformationServicesLicense amsl:PDA amsl:PPV amsl:Unknown ) ;
    rdfs:seeAlso "ERMI terms: _Acquisition Note_ (cf. https://old.diglib.org/pubs/dlf102/ERMFINAL.pdf, p. 138)" .

amsl:AllianceLicense a amsl:AcqNote ;
    rdfs:label "Allianzlizenz"@de ,
        "alliance license"@en .

amsl:OACharges a amsl:AcqNote ;
    rdfs:label "OA-Kosten"@de ,
        "OA charges"@en ;
    rdfs:comment "Open Access-Kosten"@de ,
        "Open Access Charges"@en .
       
amsl:ConsortialLicense a amsl:AcqNote ;
    rdfs:label "Konsortiallizenz"@de ,
        "consortial license"@en .  
        
amsl:DedicatedLicense a amsl:AcqNote ;
    rdfs:label "Eigene Lizenz"@de ,
        "dedicated license"@en .
                
amsl:Gift a amsl:AcqNote ;
    rdfs:label "Geschenk"@de ,
        "gift"@en .        
        
amsl:NationalLicense a amsl:AcqNote ;
    rdfs:label "Nationallizenz"@de ,
        "National license"@en .

amsl:PDA a amsl:AcqNote ;
    rdfs:label "Patron Driven Acquisiton"@de ,
        "patron driven acquisiton"@en .
        
amsl:PPV a amsl:AcqNote ;
    rdfs:label "Pay per view / use"@de ,
        "pay per view / use"@en .          
        
amsl:Purchase a amsl:AcqNote ;
    rdfs:label "Kauf"@de ,
        "purchase"@en .       

amsl:ScientificInformationServicesLicense a amsl:AcqNote ;
    rdfs:label "FID-Lizenz"@de ,
        "scientific information services license"@en ;
    rdfs:comment "Zur Kennzeichnung von Lizenzen, die durch einen FID erworben wurden und für andere Einrichtungen nachnutzbar sind."@de .              
        
amsl:Unknown a amsl:AcqNote ;
    rdfs:label "Unbekannt"@de ,
        "unknown"@en . 


amsl:AuthMethod a owl:Class ;
    owl:oneOf ( amsl:IPCampus amsl:IPSingle amsl:IPSubnet amsl:LandP amsl:Registration amsl:Shibboleth  ) .

amsl:IPCampus a amsl:AuthMethod ;
    rdfs:label "IP-Check Campusnetz"@de ,
        "IP check campus network"@en .
        
amsl:IPSingle a amsl:AuthMethod ;
    rdfs:label "IP-Check Einzelplatz (IP: ) Campusnetz"@de ,
        "IP check single station"@en .
        
amsl:IPSubnet a amsl:AuthMethod ;
    rdfs:label "IP-Check Subnetz (von - bis)"@de ,
        "IP check subnet"@en .

amsl:LandP a amsl:AuthMethod ;
    rdfs:label "Login und Passwort"@de ,
        "login and password"@en .     
          
amsl:Registration a amsl:AuthMethod ;
    rdfs:label "Registrierung"@de ,
        "registration"@en .
        
amsl:Shibboleth a amsl:AuthMethod ;
    rdfs:label "Shibboleth"@de ,
    	"shibboleth"@en .
 



amsl:BibliographicMimeType a owl:Class ;
    rdfs:subClassOf dct:MediaTypeOrExtent ;
    owl:oneOf (<urn:mimetype:application/marc> <urn:mimetype:application/marcxml+xml>) .

amsl:DownloadHTTP a gr:DeliveryMethod ;
    rdfs:label "HTTP Download"@de ,
        "HTTP download"@en .

amsl:DownloadFTP a gr:DeliveryMethod ;
    rdfs:label "FTP Download"@de ,
        "FTP download"@en .

amsl:DownloadOAI a gr:DeliveryMethod ;
    rdfs:label "OAI Download"@de ,
        "OAI download"@en .

amsl:DownloadAPI a gr:DeliveryMethod ;
    rdfs:label "API Download"@de ,
        "API download"@en .



        
amsl:Boolean a owl:Class ;
    	rdfs:subClassOf amsl:ExtendedBoolean ;
	owl:oneOf ( amsl:Yes amsl:No ) .  
	
amsl:Yes a amsl:Boolean ;
    rdfs:label "Ja"@de ,
        "yes"@en . 
        
amsl:No a amsl:Boolean ;
    rdfs:label "Nein"@de ,
        "no"@en .	    




amsl:CoverageDepth a owl:Class ;
    owl:oneOf ( amsl:FulltextCoverage amsl:SelectedArticlesCoverage amsl:AbstractCoverage ) .


amsl:FulltextCoverage a amsl:CoverageDepth ;
    rdfs:label "Volltext"@de , 
        "full text"@en .

amsl:SelectedArticlesCoverage a amsl:CoverageDepth ;
    rdfs:label "Ausgewählte Artikel"@de ,
        "selected articles"@en .

amsl:AbstractCoverage a amsl:CoverageDepth ;
    rdfs:label "Abstracts"@de ,
        "abstracts"@en .




amsl:DBType a owl:Class ;
    owl:oneOf ( amsl:EmpirDB amsl:FactDB amsl:IndexDB amsl:RealtimeDB amsl:StrucDB amsl:FulltextDB amsl:AbstrDB amsl:PicDB ) . 

amsl:AbstrDB  a amsl:DBType ;
    rdfs:label "Abstractdatenbank"@de ,
        "abstracts database"@en .
        
amsl:EmpirDB a amsl:DBType ;
    rdfs:label "empirische Datenbank"@de ,
        "empiric database"@en .

amsl:FactDB a amsl:DBType ;
    rdfs:label "Faktendatenbank"@de ,
        "facts database"@en .
                
amsl:FulltextDB a amsl:DBType ;
    rdfs:label "Volltextdatenbank"@de ,
        "fulltext database"@en .

amsl:IndexDB a amsl:DBType ;
    rdfs:label "Indexdatenbank"@de ,
        "index database"@en .
        
amsl:PicDB a amsl:DBType ;
    rdfs:label "Bilddatenbank"@de ,
        "picture database"@en .
        
amsl:RealtimeDB a amsl:DBType ;
    rdfs:label "Realtime Datenbank"@de ,
        "realtime database"@en .
        
amsl:StrucDB a amsl:DBType ;
    rdfs:label "Strukturdatenbank"@de ,
        "structure database"@en .  
              

 
        
amsl:ERType  a owl:Class ;
    owl:oneOf (amsl:Database amsl:Ebook  amsl:EbookPackage amsl:Ejournal amsl:EjournalPackage amsl:Metadata amsl:PrintPlusOnlineBook amsl:PrintPlusOnlineJournal ) .       

amsl:Database a amsl:ERType ;
    rdfs:label "Datenbank"@de ,
        "database"@en .        

amsl:Ebook a amsl:ERType ;
    rdfs:label "E-Book"@de ,
        "e-book"@en .

amsl:EbookPackage a amsl:ERType ;
    rdfs:label "E-Book Paket"@de ,
        "e-book package"@en . 
        
amsl:Ejournal a amsl:ERType ;
    rdfs:label "E-Journal"@de ,
        "e-journal"@en .
        
amsl:EjournalPackage a amsl:ERType ;
    rdfs:label "E-Journals-Paket"@de ,
        "e-journal package"@en .

amsl:Metadata a amsl:ERType ;
    rdfs:label "Metadaten"@de ,
        "metadata"@en .
        
amsl:PrintPlusOnlineBook a amsl:ERType ;
    rdfs:label "Print + Online (Buch)"@de ,
        "print + online (book)"@en .

amsl:PrintPlusOnlineJournal a amsl:ERType ;
    rdfs:label "Print + Online (Zeitschrift)"@de ,
        "print + online (journal)"@en .

 



amsl:ExtendedBoolean  a owl:Class ;
    owl:oneOf (  amsl:Yes amsl:No amsl:Undetermined ) .
        
amsl:Undetermined a amsl:ExtendedBoolean ;
    rdfs:label "Nicht festgelegt"@de ,
        "undetermined"@en .
 


 
amsl:LicenseTerm a owl:Class ;
    owl:oneOf ( amsl:NotApplicable amsl:SilentUninterpreted amsl:ProhibitedInterpreted  amsl:ProhibitedExplicit amsl:PermittedInterpreted  amsl:PermittedExplicit ) .
        
amsl:NotApplicable a amsl:LicenseTerm ;
    rdfs:label "Nicht zutreffend"@de ,
        "not applicable"@en .
 
amsl:PermittedExplicit a amsl:LicenseTerm ;
    rdfs:label "Zulässig (explizit)"@de ,
        "permitted (explicit)"@en .
                
amsl:PermittedInterpreted a amsl:LicenseTerm ;
    rdfs:label "Zulässig (Auslegung)"@de ,
        "permitted (interpreted)"@en .

amsl:ProhibitedExplicit a amsl:LicenseTerm ;
    rdfs:label "Verboten (explizit)"@de ,
        "prohibited (explicit)"@en .  
              
amsl:ProhibitedInterpreted a amsl:LicenseTerm ;
    rdfs:label "Verboten (Auslegung)"@de ,
        "prohibited (interpreted)"@en .
        
amsl:SilentUninterpreted a amsl:LicenseTerm ;
    rdfs:label "Unerwähnt"@de ,
        "unmentioned"@en .
          
 


amsl:LicenseType a owl:Class ;
    owl:oneOf ( amsl:Faculty amsl:CampusWithoutVPN amsl:Single amsl:Campus amsl:NetworkIndependent amsl:ScientificInformationServicesSpecific ) .               

amsl:Campus a amsl:LicenseType ;
    rdfs:label "Campuslizenz"@de ,
        "campus license"@en .
       
amsl:CampusWithoutVPN a amsl:LicenseType ;
    rdfs:label "Campuslizenz ohne VPN-Zugang"@de ,
        "campus license without VPN"@en .
        
amsl:Faculty a amsl:LicenseType ;
    rdfs:label "Fakultätslizenz (Class C Subnetz)"@de ,
        "faculty license"@en .     

amsl:ScientificInformationServicesSpecific a amsl:LicenseType ;
    rdfs:label "FID-spezifisch"@de ,
        "Scientific Information Services specific"@en ;
    rdfs:comment "Die Lizenz ist für den FID-spezifisch definierten Nutzerkreis gültig."@de .

amsl:NetworkIndependent a amsl:LicenseType ;
    rdfs:label "netzunabhängig"@de ,
        "network independent"@en .
        
amsl:Single a amsl:LicenseType ;
    rdfs:label "Einzelplatzlizenz"@de ,
        "single-position license"@en .  
 



 
amsl:Month a owl:DeprecatedClass ;
    owl:oneOf ( amsl:January amsl:February amsl:March amsl:April amsl:May amsl:June amsl:July amsl:August amsl:September amsl:October amsl:November amsl:December ) ;
    owl:deprecated "true"^^xsd:boolean .
              
amsl:January rdfs:label "Januar"@de ,
        "January"@en ;
    owl:deprecated "true"^^xsd:boolean .
        
amsl:February rdfs:label "Februar"@de ,
        "February"@en ;
    owl:deprecated "true"^^xsd:boolean .

amsl:March rdfs:label "März"@de ,
        "March"@en ;
    owl:deprecated "true"^^xsd:boolean .
        
amsl:April rdfs:label "April"@de ,
        "April"@en ;
    owl:deprecated "true"^^xsd:boolean .
        
amsl:May rdfs:label "Mai"@de ,
        "May"@en ;
    owl:deprecated "true"^^xsd:boolean .      

amsl:June rdfs:label "Juni"@de ,
        "June"@en ;
    owl:deprecated "true"^^xsd:boolean .

amsl:July rdfs:label "Juli"@de ,
        "July"@en ;
    owl:deprecated "true"^^xsd:boolean .
        
amsl:August rdfs:label "August"@de ,
        "August"@en ;
    owl:deprecated "true"^^xsd:boolean .
   
amsl:September rdfs:label "September"@de ,
        "September"@en   ;
    owl:deprecated "true"^^xsd:boolean .
        
amsl:October rdfs:label "Oktober"@de ,
        "October"@en ;
    owl:deprecated "true"^^xsd:boolean . 
        
amsl:November rdfs:label "November"@de ,
        "November"@en ;
    owl:deprecated "true"^^xsd:boolean .              
        
amsl:December rdfs:label "Dezember"@de ,
        "December"@en ;
    owl:deprecated "true"^^xsd:boolean .        




      
amsl:OrganizationType a owl:Class ;
    owl:oneOf ( amsl:Consortium amsl:Enterprise amsl:Library ) .        

amsl:Consortium a amsl:OrganizationType ;
    rdfs:label "Konsortium"@de ,
        "consortium"@en ;
    rdfs:seeAlso "ERMI terms: _Consortium Entity_ (cf. https://old.diglib.org/pubs/dlf102/ERMFINAL.pdf, p. 199)" .

amsl:Enterprise a amsl:OrganizationType ;
    rdfs:label "Unternehmen"@de ,
        "enterprise"@en .   
             
amsl:Library a amsl:OrganizationType ;
    rdfs:label "Bibliothek"@de ,
        "library"@en ;
    rdfs:seeAlso "ERMI terms: _Library Entity_ (cf. https://old.diglib.org/pubs/dlf102/ERMFINAL.pdf, p. 202)" .
        
 


amsl:PaymentPeriod a owl:Class ;
    owl:oneOf (amsl:PaymentInAdvance amsl:PaymentInLicensingYear) .

amsl:PaymentInAdvance a amsl:PaymentPeriod ;
    rdfs:label "Zahlung im Voraus"@de ,
        "payment in advance"@en .

amsl:PaymentInLicensingYear a amsl:PaymentPeriod ;
    rdfs:label "Zahlung im Lizenzjahr"@de ,
        "payment in licensing year"@en .


amsl:SolrShard a owl:Class .


amsl:UserGroup a owl:Class ;
    rdfs:seeAlso "ERMI terms: _User Group Entity_ (cf. https://old.diglib.org/pubs/dlf102/ERMFINAL.pdf, p. 176)" ; 
    owl:oneOf ( amsl:TeachingHospitals  amsl:Staff amsl:Students  amsl:UniMember amsl:WalkIns ) .
    
amsl:Staff a amsl:UserGroup ;
    rdfs:label "Mitarbeiter"@de ,
        "staff"@en .
        
amsl:Students a amsl:UserGroup ;
    rdfs:label "Studierende"@de ,
        "students"@en .
        
amsl:TeachingHospitals a amsl:UserGroup ;
    rdfs:label "Lehrbeauftrage Lehrkrankenhäuser"@de ,
        "teaching hospitals"@en .    

amsl:UniMember a amsl:UserGroup ;
    rdfs:label "Uni-Angehörige"@de ,
        "university members"@en .
                    
amsl:WalkIns a amsl:UserGroup ;
    rdfs:label "Walk-Ins"@de ,
        "walk Ins"@en .



               
amsl:ShibbolethImplStatus a owl:Class ;
    owl:oneOf ( amsl:Inquired amsl:Prospected amsl:InProcess amsl:Implemented amsl:Impossible   ) .

amsl:MetadataSourceImplStatus a owl:Class ;
    owl:oneOf   (amsl:Wish amsl:Inquired  amsl:InProcess amsl:Trial amsl:Active amsl:Cancelled amsl:Impossible ) .

amsl:ERStatus a owl:Class ;
    owl:oneOf ( amsl:Active amsl:Cancelled  amsl:Trial amsl:Wish  ) ;
    rdfs:seeAlso "ERMI terms: _Electronic Resource Status_ (cf. https://old.diglib.org/pubs/dlf102/ERMFINAL.pdf, p. 138)" .

amsl:WorkflowStatus a owl:Class ;
    owl:oneOf ( amsl:Inquired amsl:Renewed amsl:NotRenewed )   ;
    rdfs:seeAlso "ERMI terms: _Renewal Status_ (cf. https://old.diglib.org/pubs/dlf102/ERMFINAL.pdf, p. 138)" .


amsl:Active a amsl:ERStatus , amsl:MetadataSourceImplStatus ;
    rdfs:label "Aktiv"@de ,
        "active"@en ;
    rdfs:seeAlso "ERMI terms value: _Active_ for term _Electronic Resource Status_ (cf. https://old.diglib.org/pubs/dlf102/ERMFINAL.pdf, p. 138)" .
            
amsl:CancellationNominee a amsl:ERStatus ;
    rdfs:label "Abbestellkandidat"@de ,
        "nominee for cancellation"@en ;
    owl:deprecated "true"^^xsd:boolean .
        
amsl:Cancelled a amsl:ERStatus , amsl:MetadataSourceImplStatus ;
    rdfs:label "Abbestellt / beendet"@de ,
        "cancelled / terminated"@en ;
    rdfs:seeAlso "ERMI terms value: Retired for term _Electronic Resource Status_ (cf. https://old.diglib.org/pubs/dlf102/ERMFINAL.pdf, p. 138)" .   

amsl:Implemented a amsl:ShibbolethImplStatus ;
    rdfs:label "Implementiert"@de ,
        "implemented"@en ;
    rdfs:seeAlso "ERMI terms value: _Done_ for term _Processing Workflow Entity In-Process Group_ (cf. https://old.diglib.org/pubs/dlf102/ERMFINAL.pdf, p. 195 f.)" .

amsl:Impossible a amsl:ShibbolethImplStatus , amsl:MetadataSourceImplStatus ;
    rdfs:label "Nicht möglich"@de ,
        "not possible"@en ;
    rdfs:seeAlso "ERMI terms value: _Not Applicable_ (cf. https://old.diglib.org/pubs/dlf102/ERMFINAL.pdf, p. 195 f.)" .

amsl:InProcess a amsl:ShibbolethImplStatus , amsl:MetadataSourceImplStatus ;
    rdfs:label "In Bearbeitung (techn.)"@de ,
        "in process (techn.)"@en ;
    rdfs:comment "Wird momentan technisch bearbeitet."@de , "Is being technically processed"@en ;
    rdfs:seeAlso "ERMI terms value: _In Process_ for term _Processing Workflow Entity In-Process Group_ (cf. https://old.diglib.org/pubs/dlf102/ERMFINAL.pdf, p. 195 f.)" .

amsl:Inquired a amsl:ShibbolethImplStatus , amsl:MetadataSourceImplStatus , amsl:WorkflowStatus ;
    rdfs:label "Angefragt / In Verhandlung"@de ,
        "inquired / in negotiation"@en .

amsl:NotRenewed a amsl:WorkflowStatus ;
    rdfs:label "Nicht Verlängert"@de ,
        "not renewed"@en ;
    rdfs:seeAlso "ERMI terms value: _Cancelled_ for term _Renewal Status_ (cf. https://old.diglib.org/pubs/dlf102/ERMFINAL.pdf, p. 143)" .
        
amsl:Prospected a amsl:ShibbolethImplStatus  ;
    rdfs:label "In Aussicht"@de ,
        "prospected"@en .

amsl:Renewed a amsl:WorkflowStatus ;
    rdfs:label "Verlängert"@de ,
        "renewed"@en ;
    rdfs:seeAlso "ERMI terms value: _Renewed_ for term _Renewal Status_ (cf. https://old.diglib.org/pubs/dlf102/ERMFINAL.pdf, p. 143)" .
       
amsl:Trial a amsl:ERStatus , amsl:MetadataSourceImplStatus ;
    rdfs:label "Test"@de ,
        "trial"@en ;
    rdfs:seeAlso "ERMI terms value: _On Trial_ for term _Electronic Resource Status_ (cf. https://old.diglib.org/pubs/dlf102/ERMFINAL.pdf, p. 138)" .

amsl:Wish a amsl:ERStatus , amsl:MetadataSourceImplStatus ;
    rdfs:label "Wunsch"@de ,
        "wish"@en ;
    rdfs:seeAlso "ERMI terms value: _New request_ for term _Electronic Resource Status_ (cf. https://old.diglib.org/pubs/dlf102/ERMFINAL.pdf, p. 138)" .  


